<?xml version="1.0"?>


<!DOCTYPE rdf:RDF [
    <!ENTITY owl "http://www.w3.org/2002/07/owl#" >
    <!ENTITY xsd "http://www.w3.org/2001/XMLSchema#" >
    <!ENTITY rdfs "http://www.w3.org/2000/01/rdf-schema#" >
    <!ENTITY rdf "http://www.w3.org/1999/02/22-rdf-syntax-ns#" >
]>


<rdf:RDF xmlns="http://dendro.fe.up.pt/ontology/gravimetry#"
     xml:base="http://dendro.fe.up.pt/ontology/gravimetry"
     xmlns:rdfs="http://www.w3.org/2000/01/rdf-schema#"
     xmlns:owl="http://www.w3.org/2002/07/owl#"
     xmlns:xsd="http://www.w3.org/2001/XMLSchema#"
     xmlns:rdf="http://www.w3.org/1999/02/22-rdf-syntax-ns#">
    <owl:Ontology rdf:about="http://dendro.fe.up.pt/ontology/gravimetry">
        <owl:imports rdf:resource="http://dendro.fe.up.pt/ontology/research"/>
        <owl:versionIRI rdf:resource="http:/dendro.fe.up.pt/ontology/gravimetry/1.1"/>
    </owl:Ontology>
    


    <!-- 
    ///////////////////////////////////////////////////////////////////////////////////////
    //
    // Data properties
    //
    ///////////////////////////////////////////////////////////////////////////////////////
     -->

    


    <!-- http://dendro.fe.up.pt/ontology/BIODIV/0.1#resolutionDistance -->

    <owl:DatatypeProperty rdf:about="http://dendro.fe.up.pt/ontology/BIODIV/0.1#resolutionDistance">
        <rdfs:label>Resolution Distance</rdfs:label>
        <rdfs:isDefinedBy>Inspire Metadata Regulation. http://eur-lex.europa.eu/legal-content/EN/ALL/?uri=CELEX:32008R1205</rdfs:isDefinedBy>
        <rdfs:comment>Refers to the level of detail of the data set. It shall be expressed as a set of zero to many resolution distances (typically for gridded data and imagery-derived products).</rdfs:comment>
        <rdfs:subPropertyOf rdf:resource="http://dendro.fe.up.pt/ontology/research#measurement"/>
    </owl:DatatypeProperty>
    


    <!-- http://dendro.fe.up.pt/ontology/BIODIV/0.1#temporalExtentEndingDate -->

    <owl:DatatypeProperty rdf:about="http://dendro.fe.up.pt/ontology/BIODIV/0.1#temporalExtentEndingDate">
        <rdfs:label>Temporal Extent Ending Date</rdfs:label>
        <rdfs:comment>The temporal ending date over which the dataset was acquired.</rdfs:comment>
        <rdfs:domain rdf:resource="http://dendro.fe.up.pt/ontology/gravimetry#AerialGravimetry"/>
    </owl:DatatypeProperty>
    


    <!-- http://dendro.fe.up.pt/ontology/BIODIV/0.1#temporalExtentStartingDate -->

    <owl:DatatypeProperty rdf:about="http://dendro.fe.up.pt/ontology/BIODIV/0.1#temporalExtentStartingDate">
        <rdfs:label>Temporal Extent Starting Date</rdfs:label>
        <rdfs:comment>The temporal starting data over which the dataset was acquired.</rdfs:comment>
        <rdfs:domain rdf:resource="http://dendro.fe.up.pt/ontology/gravimetry#AerialGravimetry"/>
    </owl:DatatypeProperty>
    


    <!-- http://dendro.fe.up.pt/ontology/gravimetry#altitudeDatumName -->

    <owl:DatatypeProperty rdf:about="http://dendro.fe.up.pt/ontology/gravimetry#altitudeDatumName">
        <rdfs:label>Altitude Datum Name</rdfs:label>
        <rdfs:comment>The identification given to the surface taken as the surface of
reference from which altitudes are measured</rdfs:comment>
        <rdfs:isDefinedBy>Content Standard for Digital Geospatial Metadata https://www.fgdc.gov/standards/projects/FGDC-standards-projects/metadata/base-metadata/v2_0698.pdf</rdfs:isDefinedBy>
        <rdfs:domain rdf:resource="http://dendro.fe.up.pt/ontology/gravimetry#AerialGravimetry"/>
    </owl:DatatypeProperty>
    


    <!-- http://dendro.fe.up.pt/ontology/gravimetry#altitudeDistanceUnits -->

    <owl:DatatypeProperty rdf:about="http://dendro.fe.up.pt/ontology/gravimetry#altitudeDistanceUnits">
        <rdfs:label>Altitude Distance Units</rdfs:label>
        <rdfs:isDefinedBy>Content Standard for Digital Geospatial Metadata https://www.fgdc.gov/standards/projects/FGDC-standards-projects/metadata/base-metadata/v2_0698.pdf</rdfs:isDefinedBy>
        <rdfs:comment>Units in which altitudes are recorded.</rdfs:comment>
        <rdfs:domain rdf:resource="http://dendro.fe.up.pt/ontology/gravimetry#AerialGravimetry"/>
    </owl:DatatypeProperty>
    


    <!-- http://dendro.fe.up.pt/ontology/gravimetry#altitudeEncodingMethods -->

    <owl:DatatypeProperty rdf:about="http://dendro.fe.up.pt/ontology/gravimetry#altitudeEncodingMethods">
        <rdfs:label>Altitude Encoding Methods</rdfs:label>
        <rdfs:isDefinedBy>Content Standard for Digital Geospatial Metadata https://www.fgdc.gov/standards/projects/FGDC-standards-projects/metadata/base-metadata/v2_0698.pdf</rdfs:isDefinedBy>
        <rdfs:comment>The means used to encode the altitudes.</rdfs:comment>
        <rdfs:domain rdf:resource="http://dendro.fe.up.pt/ontology/gravimetry#AerialGravimetry"/>
        <rdfs:subPropertyOf rdf:resource="http://dendro.fe.up.pt/ontology/research#method"/>
    </owl:DatatypeProperty>
    


    <!-- http://dendro.fe.up.pt/ontology/gravimetry#altitudeResolution -->

    <owl:DatatypeProperty rdf:about="http://dendro.fe.up.pt/ontology/gravimetry#altitudeResolution">
        <rdfs:label>Altitude Resolution</rdfs:label>
        <rdfs:comment>The minimum distance possible between two adjacent altitude
values, expressed in Altitude Distance Units of measure.
</rdfs:comment>
        <rdfs:isDefinedBy>Content Standard for Digital Geospatial Metadata https://www.fgdc.gov/standards/projects/FGDC-standards-projects/metadata/base-metadata/v2_0698.pdf</rdfs:isDefinedBy>
        <rdfs:domain rdf:resource="http://dendro.fe.up.pt/ontology/gravimetry#AerialGravimetry"/>
        <rdfs:subPropertyOf rdf:resource="http://dendro.fe.up.pt/ontology/research#measurement"/>
    </owl:DatatypeProperty>
    


    <!-- http://dendro.fe.up.pt/ontology/gravimetry#altitudeSystemDefinition -->

    <owl:DatatypeProperty rdf:about="http://dendro.fe.up.pt/ontology/gravimetry#altitudeSystemDefinition">
        <rdfs:label>Altitude System Definition</rdfs:label>
        <rdfs:isDefinedBy>Content Standard for Digital Geospatial Metadata https://www.fgdc.gov/standards/projects/FGDC-standards-projects/metadata/base-metadata/v2_0698.pdf</rdfs:isDefinedBy>
        <rdfs:comment>The reference frame or system from which altitudes (elevations)
are measured. The term &quot;altitude&quot;&apos; is used instead of the common term &quot;elevation&quot; to conform to the terminology in Federal Information Processing Standards 70-1 and 173.
</rdfs:comment>
        <rdfs:domain rdf:resource="http://dendro.fe.up.pt/ontology/gravimetry#AerialGravimetry"/>
    </owl:DatatypeProperty>
    


    <!-- http://dendro.fe.up.pt/ontology/gravimetry#beginningTime -->

    <owl:DatatypeProperty rdf:about="http://dendro.fe.up.pt/ontology/gravimetry#beginningTime">
        <rdfs:label>Beginning Time</rdfs:label>
        <rdfs:comment>The first hour (an optionally minute, or minute and second) of the day for the event.</rdfs:comment>
        <rdfs:isDefinedBy>Content Standard for Digital Geospatial Metadata https://www.fgdc.gov/standards/projects/FGDC-standards-projects/metadata/base-metadata/v2_0698.pdf</rdfs:isDefinedBy>
    </owl:DatatypeProperty>
    


    <!-- http://dendro.fe.up.pt/ontology/gravimetry#endingTime -->

    <owl:DatatypeProperty rdf:about="http://dendro.fe.up.pt/ontology/gravimetry#endingTime">
        <rdfs:label>Ending Time</rdfs:label>
        <rdfs:isDefinedBy>Content Standard for Digital Geospatial Metadata https://www.fgdc.gov/standards/projects/FGDC-standards-projects/metadata/base-metadata/v2_0698.pdf</rdfs:isDefinedBy>
        <rdfs:comment>The last hour (an optionally minute, or minute and second) of the day for the event.</rdfs:comment>
        <rdfs:domain rdf:resource="http://dendro.fe.up.pt/ontology/BIODIV/0.1#TemporalReference"/>
        <rdfs:domain rdf:resource="http://dendro.fe.up.pt/ontology/gravimetry#AerialGravimetry"/>
    </owl:DatatypeProperty>
    


    <!-- http://dendro.fe.up.pt/ontology/gravimetry#geographicBoundingBox -->

    <owl:DatatypeProperty rdf:about="http://dendro.fe.up.pt/ontology/gravimetry#geographicBoundingBox">
        <rdfs:label>Geographic Bounding Box</rdfs:label>
        <rdfs:isDefinedBy>Inspire Metadata Regulation. http://eur-lex.europa.eu/legal-content/EN/ALL/?uri=CELEX:32008R1205</rdfs:isDefinedBy>
        <rdfs:comment>This is the extent of the resource in the geographic space, given as a bounding box. The bounding box shall be expressed with westbound and eastbound longitudes, and southbound and northbound latitudes in decimal degrees, with a precision of at least two decimals.</rdfs:comment>
        <rdfs:domain rdf:resource="http://dendro.fe.up.pt/ontology/BIODIV/0.1#GeographicLocation"/>
        <rdfs:domain rdf:resource="http://dendro.fe.up.pt/ontology/gravimetry#AerialGravimetry"/>
    </owl:DatatypeProperty>
    


    <!-- 
    ///////////////////////////////////////////////////////////////////////////////////////
    //
    // Classes
    //
    ///////////////////////////////////////////////////////////////////////////////////////
     -->

    


    <!-- http://dendro.fe.up.pt/ontology/BIODIV/0.1#GeographicLocation -->

    <owl:Class rdf:about="http://dendro.fe.up.pt/ontology/BIODIV/0.1#GeographicLocation"/>
    


    <!-- http://dendro.fe.up.pt/ontology/BIODIV/0.1#TemporalReference -->

    <owl:Class rdf:about="http://dendro.fe.up.pt/ontology/BIODIV/0.1#TemporalReference"/>
    


    <!-- http://dendro.fe.up.pt/ontology/gravimetry#AerialGravimetry -->

    <owl:Class rdf:about="http://dendro.fe.up.pt/ontology/gravimetry#AerialGravimetry">
        <rdfs:label>Aerial Gravimetry</rdfs:label>
        <rdfs:subClassOf rdf:resource="http://dendro.fe.up.pt/ontology/research#Experiment"/>
    </owl:Class>
</rdf:RDF>



<!-- Generated by the OWL API (version 3.4.2) http://owlapi.sourceforge.net -->

