<?xml version="1.0"?>
<rdf:RDF xmlns="http://dendro.fe.up.pt/ontology/tvu/"
     xml:base="http://dendro.fe.up.pt/ontology/tvu/"
     xmlns:tvu="http://dendro.fe.up.pt/ontology/tvu#"
     xmlns:rdf="http://www.w3.org/1999/02/22-rdf-syntax-ns#"
     xmlns:terms="http://purl.org/dc/terms/"
     xmlns:owl="http://www.w3.org/2002/07/owl#"
     xmlns:ns="http://creativecommons.org/ns#"
     xmlns:untitled-ontology-98="http://www.semanticweb.org/sara-/ontologies/2017/3/untitled-ontology-98#"
     xmlns:xml="http://www.w3.org/XML/1998/namespace"
     xmlns:xsd="http://www.w3.org/2001/XMLSchema#"
     xmlns:rdfs="http://www.w3.org/2000/01/rdf-schema#"
     xmlns:vann="http://purl.org/vocab/vann/"
     xmlns:foaf="http://xmlns.com/foaf/0.1/">
    <owl:Ontology rdf:about="http://dendro.fe.up.pt/ontology/tvu">
        <owl:imports rdf:resource="http://dbpedia.org/ontology/"/>
        <owl:imports rdf:resource="http://www.ebu.ch/metadata/ontologies/ebucore/ebucore"/>
        <untitled-ontology-98:license>Creative Commons Attribution-NonCommercial_ShareAlike (CC-BY-NC-SA)</untitled-ontology-98:license>
        <untitled-ontology-98:creator>Sara Oliveira</untitled-ontology-98:creator>
        <rdfs:seeAlso>DBpedia Ontology http://dbpedia.org/ontology/
Dublin Core http://dublincore.org/documents/dces/ 
EBU Ontology (ebucore) http://www.ebu.ch/metadata/ontologies/ebucore/ebucore
Programmes Ontology http://purl.org/ontology/po/
VideoMD: Video Technical Metadata Extension Schema https://www.loc.gov/standards/amdvmd/</rdfs:seeAlso>
        <untitled-ontology-98:description>A list of concepts for the description of the dataset generated in the scope of audiovisual production.</untitled-ontology-98:description>
    </owl:Ontology>
    


    <!-- 
    ///////////////////////////////////////////////////////////////////////////////////////
    //
    // Annotation properties
    //
    ///////////////////////////////////////////////////////////////////////////////////////
     -->

    


    <!-- http://dendro.fe.up.pt/ontology/tvu#creator -->

    <owl:AnnotationProperty rdf:about="http://dendro.fe.up.pt/ontology/tvu#creator"/>
    


    <!-- http://dendro.fe.up.pt/ontology/tvu#description -->

    <owl:AnnotationProperty rdf:about="http://dendro.fe.up.pt/ontology/tvu#description"/>
    


    <!-- http://dendro.fe.up.pt/ontology/tvu#license -->

    <owl:AnnotationProperty rdf:about="http://dendro.fe.up.pt/ontology/tvu#license"/>
    


    <!-- 
    ///////////////////////////////////////////////////////////////////////////////////////
    //
    // Object Properties
    //
    ///////////////////////////////////////////////////////////////////////////////////////
     -->

    


    <!-- http://dendro.fe.up.pt/ontology/tvu#contact -->

    <owl:ObjectProperty rdf:about="http://dendro.fe.up.pt/ontology/tvu#contact">
        <rdfs:subPropertyOf rdf:resource="http://www.w3.org/2002/07/owl#topObjectProperty"/>
        <rdfs:domain rdf:resource="http://www.w3.org/2002/07/owl#Thing"/>
        <rdfs:range>
            <owl:Restriction>
                <owl:onProperty rdf:resource="http://dendro.fe.up.pt/ontology/tvu#homepageOffice"/>
                <owl:someValuesFrom rdf:resource="http://www.w3.org/2001/XMLSchema#anyURI"/>
            </owl:Restriction>
        </rdfs:range>
        <rdfs:range>
            <owl:Restriction>
                <owl:onProperty rdf:resource="http://dendro.fe.up.pt/ontology/tvu#officeMailAddress"/>
                <owl:someValuesFrom rdf:resource="http://www.w3.org/2001/XMLSchema#string"/>
            </owl:Restriction>
        </rdfs:range>
        <rdfs:range>
            <owl:Restriction>
                <owl:onProperty rdf:resource="http://dendro.fe.up.pt/ontology/tvu#telephoneOffice"/>
                <owl:someValuesFrom rdf:resource="http://www.w3.org/2001/XMLSchema#integer"/>
            </owl:Restriction>
        </rdfs:range>
    </owl:ObjectProperty>
    


    <!-- http://dendro.fe.up.pt/ontology/tvu#date -->

    <owl:ObjectProperty rdf:about="http://dendro.fe.up.pt/ontology/tvu#date">
        <rdfs:subPropertyOf rdf:resource="http://www.w3.org/2002/07/owl#topObjectProperty"/>
        <rdfs:domain rdf:resource="http://www.w3.org/2002/07/owl#Thing"/>
        <rdfs:range>
            <owl:Restriction>
                <owl:onProperty rdf:resource="http://dendro.fe.up.pt/ontology/tvu#endDateAndTime"/>
                <owl:someValuesFrom rdf:resource="http://www.w3.org/2001/XMLSchema#integer"/>
            </owl:Restriction>
        </rdfs:range>
        <rdfs:range>
            <owl:Restriction>
                <owl:onProperty rdf:resource="http://dendro.fe.up.pt/ontology/tvu#eventEndDate"/>
                <owl:someValuesFrom rdf:resource="http://www.w3.org/2001/XMLSchema#integer"/>
            </owl:Restriction>
        </rdfs:range>
        <rdfs:range>
            <owl:Restriction>
                <owl:onProperty rdf:resource="http://dendro.fe.up.pt/ontology/tvu#eventStartDate"/>
                <owl:someValuesFrom rdf:resource="http://www.w3.org/2001/XMLSchema#integer"/>
            </owl:Restriction>
        </rdfs:range>
        <rdfs:range>
            <owl:Restriction>
                <owl:onProperty rdf:resource="http://dendro.fe.up.pt/ontology/tvu#startDateAndTime"/>
                <owl:someValuesFrom rdf:resource="http://www.w3.org/2001/XMLSchema#integer"/>
            </owl:Restriction>
        </rdfs:range>
    </owl:ObjectProperty>
    


    <!-- 
    ///////////////////////////////////////////////////////////////////////////////////////
    //
    // Data properties
    //
    ///////////////////////////////////////////////////////////////////////////////////////
     -->

    


    <!-- http://dbpedia.org/ontology/comment -->

    <owl:DatatypeProperty rdf:about="http://dbpedia.org/ontology/comment">
        <owl:equivalentProperty rdf:resource="http://dendro.fe.up.pt/ontology/tvu#comment"/>
    </owl:DatatypeProperty>
    


    <!-- http://dbpedia.org/ontology/dateLastUpdated -->

    <owl:DatatypeProperty rdf:about="http://dbpedia.org/ontology/dateLastUpdated">
        <owl:equivalentProperty rdf:resource="http://dendro.fe.up.pt/ontology/tvu#dateLastUpdated"/>
    </owl:DatatypeProperty>
    


    <!-- http://dbpedia.org/ontology/endDateTime -->

    <owl:DatatypeProperty rdf:about="http://dbpedia.org/ontology/endDateTime">
        <owl:equivalentProperty rdf:resource="http://dendro.fe.up.pt/ontology/tvu#endDateAndTime"/>
    </owl:DatatypeProperty>
    


    <!-- http://dbpedia.org/ontology/episodeNumber -->

    <owl:DatatypeProperty rdf:about="http://dbpedia.org/ontology/episodeNumber">
        <owl:equivalentProperty rdf:resource="http://dendro.fe.up.pt/ontology/tvu#episodeNumber"/>
    </owl:DatatypeProperty>
    


    <!-- http://dbpedia.org/ontology/office -->

    <owl:DatatypeProperty rdf:about="http://dbpedia.org/ontology/office">
        <owl:equivalentProperty rdf:resource="http://dendro.fe.up.pt/ontology/tvu#officeMailAddress"/>
    </owl:DatatypeProperty>
    


    <!-- http://dbpedia.org/ontology/publicationDate -->

    <owl:DatatypeProperty rdf:about="http://dbpedia.org/ontology/publicationDate">
        <owl:equivalentProperty rdf:resource="http://dendro.fe.up.pt/ontology/tvu#publicationDate"/>
    </owl:DatatypeProperty>
    


    <!-- http://dbpedia.org/ontology/quotation -->

    <owl:DatatypeProperty rdf:about="http://dbpedia.org/ontology/quotation">
        <owl:equivalentProperty rdf:resource="http://dendro.fe.up.pt/ontology/tvu#quotation"/>
    </owl:DatatypeProperty>
    


    <!-- http://dbpedia.org/ontology/startDateTime -->

    <owl:DatatypeProperty rdf:about="http://dbpedia.org/ontology/startDateTime">
        <owl:equivalentProperty rdf:resource="http://dendro.fe.up.pt/ontology/tvu#startDateAndTime"/>
    </owl:DatatypeProperty>
    


    <!-- http://dendro.fe.up.pt/ontology/tvu#actor -->

    <owl:DatatypeProperty rdf:about="http://dendro.fe.up.pt/ontology/tvu#actor">
        <rdfs:subPropertyOf rdf:resource="http://www.w3.org/2002/07/owl#topDataProperty"/>
        <rdfs:domain rdf:resource="http://dendro.fe.up.pt/ontology/tvu#AudiovisualContent"/>
        <rdfs:range rdf:resource="http://www.w3.org/2001/XMLSchema#string"/>
        <rdfs:comment>The person who plays the role of a character in the audiovisual content.</rdfs:comment>
        <rdfs:isDefinedBy>Programmes ontology http://www.bbc.co.uk/ontologies/po</rdfs:isDefinedBy>
        <rdfs:label>Actor</rdfs:label>
    </owl:DatatypeProperty>
    


    <!-- http://dendro.fe.up.pt/ontology/tvu#aspectRatio -->

    <owl:DatatypeProperty rdf:about="http://dendro.fe.up.pt/ontology/tvu#aspectRatio">
        <owl:equivalentProperty rdf:resource="http://www.ebu.ch/metadata/ontologies/ebucore/ebucore#aspectRatio"/>
        <rdfs:subPropertyOf rdf:resource="http://www.w3.org/2002/07/owl#topDataProperty"/>
        <rdfs:domain rdf:resource="http://dendro.fe.up.pt/ontology/tvu#AudiovisualContent"/>
        <rdfs:range rdf:resource="http://www.w3.org/2001/XMLSchema#integer"/>
        <rdfs:comment>The aspect ratio of a audiovisual content, describes the proportional relationship between its width and its height. Is expressed as two numbers separated by a colon (x:y)</rdfs:comment>
        <rdfs:isDefinedBy>EBU Ontology (ebucore) http://lov.okfn.org/dataset/lov/vocabs/ebucore</rdfs:isDefinedBy>
        <rdfs:label>Aspect Ratio</rdfs:label>
    </owl:DatatypeProperty>
    


    <!-- http://dendro.fe.up.pt/ontology/tvu#attachments -->

    <owl:DatatypeProperty rdf:about="http://dendro.fe.up.pt/ontology/tvu#attachments">
        <rdfs:subPropertyOf rdf:resource="http://www.w3.org/2002/07/owl#topDataProperty"/>
        <rdfs:domain rdf:resource="http://dendro.fe.up.pt/ontology/tvu#AudiovisualContent"/>
        <rdfs:range rdf:resource="http://www.w3.org/2001/XMLSchema#string"/>
        <rdfs:comment>The file related to the audiovisual content, which may take different formats (PDF, PPT, JPEG).</rdfs:comment>
        <rdfs:isDefinedBy>TVU. Vocabulary</rdfs:isDefinedBy>
        <rdfs:label>Attachments</rdfs:label>
    </owl:DatatypeProperty>
    


    <!-- http://dendro.fe.up.pt/ontology/tvu#averageBitRate -->

    <owl:DatatypeProperty rdf:about="http://dendro.fe.up.pt/ontology/tvu#averageBitRate">
        <owl:equivalentProperty rdf:resource="http://www.w3.org/ns/ma-ont#averageBitRate"/>
        <rdfs:subPropertyOf rdf:resource="http://www.w3.org/2002/07/owl#topDataProperty"/>
        <rdfs:domain rdf:resource="http://dendro.fe.up.pt/ontology/tvu#AudiovisualContent"/>
        <rdfs:range rdf:resource="http://www.w3.org/2001/XMLSchema#integer"/>
        <rdfs:comment>Refers to the average amount of data transferred per unit of time, usually measured per second, commonly for digital music or video.</rdfs:comment>
        <rdfs:isDefinedBy>EBU Ontology (ebucore) http://lov.okfn.org/dataset/lov/vocabs/ebucore</rdfs:isDefinedBy>
        <rdfs:label>Average Bit Rate</rdfs:label>
    </owl:DatatypeProperty>
    


    <!-- http://dendro.fe.up.pt/ontology/tvu#channel -->

    <owl:DatatypeProperty rdf:about="http://dendro.fe.up.pt/ontology/tvu#channel">
        <rdfs:subPropertyOf rdf:resource="http://www.w3.org/2002/07/owl#topDataProperty"/>
        <rdfs:domain rdf:resource="http://dendro.fe.up.pt/ontology/tvu#AudiovisualContent"/>
        <rdfs:range rdf:resource="http://www.w3.org/2001/XMLSchema#string"/>
        <rdfs:comment>The channel in which audiovisual content is contained.</rdfs:comment>
        <rdfs:isDefinedBy>Programmes ontology http://www.bbc.co.uk/ontologies/po</rdfs:isDefinedBy>
        <rdfs:label>Channel</rdfs:label>
    </owl:DatatypeProperty>
    


    <!-- http://dendro.fe.up.pt/ontology/tvu#chapters -->

    <owl:DatatypeProperty rdf:about="http://dendro.fe.up.pt/ontology/tvu#chapters">
        <rdfs:subPropertyOf rdf:resource="http://www.w3.org/2002/07/owl#topDataProperty"/>
        <rdfs:domain rdf:resource="http://dendro.fe.up.pt/ontology/tvu#AudiovisualContent"/>
        <rdfs:range rdf:resource="http://www.w3.org/2001/XMLSchema#string"/>
        <rdfs:comment>Identifies the chapters included in the audiovisual content, with reference to the time.</rdfs:comment>
        <rdfs:isDefinedBy>TVU. Vocabulary</rdfs:isDefinedBy>
        <rdfs:label>Chapters</rdfs:label>
    </owl:DatatypeProperty>
    


    <!-- http://dendro.fe.up.pt/ontology/tvu#codecName -->

    <owl:DatatypeProperty rdf:about="http://dendro.fe.up.pt/ontology/tvu#codecName">
        <owl:equivalentProperty rdf:resource="http://www.ebu.ch/metadata/ontologies/ebucore/ebucore#codecName"/>
        <rdfs:subPropertyOf rdf:resource="http://www.w3.org/2002/07/owl#topDataProperty"/>
        <rdfs:domain rdf:resource="http://dendro.fe.up.pt/ontology/tvu#AudiovisualContent"/>
        <rdfs:range rdf:resource="http://www.w3.org/2001/XMLSchema#string"/>
        <rdfs:comment>Information about the hardware or software which makes the storage process or files transmission lighter.</rdfs:comment>
        <rdfs:isDefinedBy>EBU Ontology (ebucore) http://lov.okfn.org/dataset/lov/vocabs/ebucore</rdfs:isDefinedBy>
        <rdfs:label>Codec Name</rdfs:label>
    </owl:DatatypeProperty>
    


    <!-- http://dendro.fe.up.pt/ontology/tvu#comment -->

    <owl:DatatypeProperty rdf:about="http://dendro.fe.up.pt/ontology/tvu#comment">
        <rdfs:subPropertyOf rdf:resource="http://www.w3.org/2002/07/owl#topDataProperty"/>
        <rdfs:domain rdf:resource="http://dendro.fe.up.pt/ontology/tvu#AudiovisualContent"/>
        <rdfs:range rdf:resource="http://www.w3.org/2001/XMLSchema#string"/>
        <rdfs:comment>Opinion or an observation made by a user.</rdfs:comment>
        <rdfs:isDefinedBy>DBpedia Ontology http://wiki.dbpedia.org/services-resources/ontology</rdfs:isDefinedBy>
        <rdfs:label>Comment</rdfs:label>
    </owl:DatatypeProperty>
    


    <!-- http://dendro.fe.up.pt/ontology/tvu#commentator -->

    <owl:DatatypeProperty rdf:about="http://dendro.fe.up.pt/ontology/tvu#commentator">
        <rdfs:subPropertyOf rdf:resource="http://www.w3.org/2002/07/owl#topDataProperty"/>
        <rdfs:domain rdf:resource="http://dendro.fe.up.pt/ontology/tvu#AudiovisualContent"/>
        <rdfs:range rdf:resource="http://www.w3.org/2001/XMLSchema#string"/>
        <rdfs:comment>Programmes ontology http://www.bbc.co.uk/ontologies/po</rdfs:comment>
        <rdfs:comment>The person who relates/comments the audiovisual contents (usually in documentaries).</rdfs:comment>
        <rdfs:label>Commentator</rdfs:label>
    </owl:DatatypeProperty>
    


    <!-- http://dendro.fe.up.pt/ontology/tvu#curator -->

    <owl:DatatypeProperty rdf:about="http://dendro.fe.up.pt/ontology/tvu#curator">
        <rdfs:subPropertyOf rdf:resource="http://www.w3.org/2002/07/owl#topDataProperty"/>
        <rdfs:domain rdf:resource="http://dendro.fe.up.pt/ontology/tvu#AudiovisualContent"/>
        <rdfs:range rdf:resource="http://www.w3.org/2001/XMLSchema#string"/>
        <rdfs:comment>The person who is responsible for making audiovisual contents available to the public and for manage the metadata associated to the audiovisual contents.</rdfs:comment>
        <rdfs:isDefinedBy>TVU. Vocabulary</rdfs:isDefinedBy>
        <rdfs:label>Curator</rdfs:label>
    </owl:DatatypeProperty>
    


    <!-- http://dendro.fe.up.pt/ontology/tvu#dataRate -->

    <owl:DatatypeProperty rdf:about="http://dendro.fe.up.pt/ontology/tvu#dataRate">
        <rdfs:subPropertyOf rdf:resource="http://www.w3.org/2002/07/owl#topDataProperty"/>
        <rdfs:domain rdf:resource="http://dendro.fe.up.pt/ontology/tvu#AudiovisualContent"/>
        <rdfs:range rdf:resource="http://www.w3.org/2001/XMLSchema#integer"/>
        <rdfs:comment>The speed at which data is transferred within the computer or between a peripheral device and computer, measured in bytes per second.</rdfs:comment>
        <rdfs:isDefinedBy>VideoMD: Video Technical Metadata Extension Schema http://hopewiki.socialhistoryportal.org/index.php/Media_Specific_Standards_for_Technical_Metadata</rdfs:isDefinedBy>
        <rdfs:label>Data Rate</rdfs:label>
    </owl:DatatypeProperty>
    


    <!-- http://dendro.fe.up.pt/ontology/tvu#dateLastUpdated -->

    <owl:DatatypeProperty rdf:about="http://dendro.fe.up.pt/ontology/tvu#dateLastUpdated">
        <rdfs:subPropertyOf rdf:resource="http://www.w3.org/2002/07/owl#topDataProperty"/>
        <rdfs:domain rdf:resource="http://dendro.fe.up.pt/ontology/tvu#AudiovisualContent"/>
        <rdfs:range rdf:resource="http://www.w3.org/2001/XMLSchema#integer"/>
        <rdfs:comment>The date at which was made the last updated to the audiovisual content.</rdfs:comment>
        <rdfs:isDefinedBy>DBpedia Ontology http://wiki.dbpedia.org/services-resources/ontology</rdfs:isDefinedBy>
        <rdfs:label>Date Last Updated</rdfs:label>
    </owl:DatatypeProperty>
    


    <!-- http://dendro.fe.up.pt/ontology/tvu#duration -->

    <owl:DatatypeProperty rdf:about="http://dendro.fe.up.pt/ontology/tvu#duration">
        <owl:equivalentProperty rdf:resource="http://www.ebu.ch/metadata/ontologies/ebucore/ebucore#eventDuration"/>
        <rdfs:subPropertyOf rdf:resource="http://www.w3.org/2002/07/owl#topDataProperty"/>
        <rdfs:domain rdf:resource="http://dendro.fe.up.pt/ontology/tvu#AudiovisualContent"/>
        <rdfs:range rdf:resource="http://www.w3.org/2001/XMLSchema#integer"/>
        <rdfs:comment>Information about the duration of a audiovisual content.</rdfs:comment>
        <rdfs:isDefinedBy>EBU Ontology (ebucore) http://lov.okfn.org/dataset/lov/vocabs/ebucore</rdfs:isDefinedBy>
        <rdfs:label>Duration</rdfs:label>
    </owl:DatatypeProperty>
    


    <!-- http://dendro.fe.up.pt/ontology/tvu#endDateAndTime -->

    <owl:DatatypeProperty rdf:about="http://dendro.fe.up.pt/ontology/tvu#endDateAndTime">
        <rdfs:subPropertyOf rdf:resource="http://www.w3.org/2002/07/owl#topDataProperty"/>
        <rdfs:domain rdf:resource="http://dendro.fe.up.pt/ontology/tvu#AudiovisualContent"/>
        <rdfs:range rdf:resource="http://www.w3.org/2001/XMLSchema#integer"/>
        <rdfs:comment>The end date and time of an event captured in the audiovisual content. Indicated to use in promotional audiovisual contents.</rdfs:comment>
        <rdfs:isDefinedBy>DBpedia Ontology http://wiki.dbpedia.org/services-resources/ontology</rdfs:isDefinedBy>
        <rdfs:label>End Date and Time</rdfs:label>
    </owl:DatatypeProperty>
    


    <!-- http://dendro.fe.up.pt/ontology/tvu#episodeNumber -->

    <owl:DatatypeProperty rdf:about="http://dendro.fe.up.pt/ontology/tvu#episodeNumber">
        <rdfs:subPropertyOf rdf:resource="http://www.w3.org/2002/07/owl#topDataProperty"/>
        <rdfs:domain rdf:resource="http://dendro.fe.up.pt/ontology/tvu#AudiovisualContent"/>
        <rdfs:range rdf:resource="http://www.w3.org/2001/XMLSchema#integer"/>
        <rdfs:comment>Identifies the episode number which is included in a premium channel.</rdfs:comment>
        <rdfs:isDefinedBy>DBpedia ontology http://wiki.dbpedia.org/services-resources/ontology</rdfs:isDefinedBy>
        <rdfs:label>Episode Number</rdfs:label>
    </owl:DatatypeProperty>
    


    <!-- http://dendro.fe.up.pt/ontology/tvu#eventEndDate -->

    <owl:DatatypeProperty rdf:about="http://dendro.fe.up.pt/ontology/tvu#eventEndDate">
        <owl:equivalentProperty rdf:resource="http://www.ebu.ch/metadata/ontologies/ebucore/ebucore#eventEndDate"/>
        <rdfs:subPropertyOf rdf:resource="http://www.w3.org/2002/07/owl#topDataProperty"/>
        <rdfs:domain rdf:resource="http://dendro.fe.up.pt/ontology/tvu#AudiovisualContent"/>
        <rdfs:range rdf:resource="http://www.w3.org/2001/XMLSchema#integer"/>
        <rdfs:comment>The end date of an event captured in the audiovisual content.</rdfs:comment>
        <rdfs:isDefinedBy>EBU Ontology (ebucore) http://lov.okfn.org/dataset/lov/vocabs/ebucore</rdfs:isDefinedBy>
        <rdfs:label>Event End Date</rdfs:label>
    </owl:DatatypeProperty>
    


    <!-- http://dendro.fe.up.pt/ontology/tvu#eventStartDate -->

    <owl:DatatypeProperty rdf:about="http://dendro.fe.up.pt/ontology/tvu#eventStartDate">
        <owl:equivalentProperty rdf:resource="http://www.ebu.ch/metadata/ontologies/ebucore/ebucore#eventStartDate"/>
        <rdfs:subPropertyOf rdf:resource="http://www.w3.org/2002/07/owl#topDataProperty"/>
        <rdfs:domain rdf:resource="http://dendro.fe.up.pt/ontology/tvu#AudiovisualContent"/>
        <rdfs:range rdf:resource="http://www.w3.org/2001/XMLSchema#integer"/>
        <rdfs:comment>The start date of an event captured in the audiovisual content.</rdfs:comment>
        <rdfs:isDefinedBy>EBU Ontology (ebucore) http://lov.okfn.org/dataset/lov/vocabs/ebucore</rdfs:isDefinedBy>
        <rdfs:label>Event Start Date</rdfs:label>
    </owl:DatatypeProperty>
    


    <!-- http://dendro.fe.up.pt/ontology/tvu#fileName -->

    <owl:DatatypeProperty rdf:about="http://dendro.fe.up.pt/ontology/tvu#fileName">
        <owl:equivalentProperty rdf:resource="http://www.ebu.ch/metadata/ontologies/ebucore/ebucore#filename"/>
        <rdfs:subPropertyOf rdf:resource="http://www.w3.org/2002/07/owl#topDataProperty"/>
        <rdfs:domain rdf:resource="http://dendro.fe.up.pt/ontology/tvu#AudiovisualContent"/>
        <rdfs:range rdf:resource="http://www.w3.org/2001/XMLSchema#string"/>
        <rdfs:comment>Is a name used to uniquely identify a computer file stored in a file system.</rdfs:comment>
        <rdfs:isDefinedBy>EBU Ontology (ebucore) http://lov.okfn.org/dataset/lov/vocabs/ebucore</rdfs:isDefinedBy>
        <rdfs:label>File Name</rdfs:label>
    </owl:DatatypeProperty>
    


    <!-- http://dendro.fe.up.pt/ontology/tvu#fileSize -->

    <owl:DatatypeProperty rdf:about="http://dendro.fe.up.pt/ontology/tvu#fileSize">
        <owl:equivalentProperty rdf:resource="http://www.ebu.ch/metadata/ontologies/ebucore/ebucore#fileSize"/>
        <rdfs:subPropertyOf rdf:resource="http://www.w3.org/2002/07/owl#topDataProperty"/>
        <rdfs:domain rdf:resource="http://dendro.fe.up.pt/ontology/tvu#AudiovisualContent"/>
        <rdfs:range rdf:resource="http://www.w3.org/2001/XMLSchema#decimal"/>
        <rdfs:comment>Is a measure of how much data a computer file contains, or, alternately, how much storage it consumes. File size is typically expressed in bytes.</rdfs:comment>
        <rdfs:isDefinedBy>EBU Ontology (ebucore) http://lov.okfn.org/dataset/lov/vocabs/ebucore</rdfs:isDefinedBy>
        <rdfs:label>File Size</rdfs:label>
    </owl:DatatypeProperty>
    


    <!-- http://dendro.fe.up.pt/ontology/tvu#frameRate -->

    <owl:DatatypeProperty rdf:about="http://dendro.fe.up.pt/ontology/tvu#frameRate">
        <owl:equivalentProperty rdf:resource="http://www.ebu.ch/metadata/ontologies/ebucore/ebucore#frameRate"/>
        <rdfs:subPropertyOf rdf:resource="http://www.w3.org/2002/07/owl#topDataProperty"/>
        <rdfs:domain rdf:resource="http://dendro.fe.up.pt/ontology/tvu#AudiovisualContent"/>
        <rdfs:range rdf:resource="http://www.w3.org/2001/XMLSchema#integer"/>
        <rdfs:comment>Is the frequency at which consecutive images are displayed in an animated display. Frame rate is usually expressed in hertz.</rdfs:comment>
        <rdfs:isDefinedBy>EBU Ontology (ebucore) http://lov.okfn.org/dataset/lov/vocabs/ebucore</rdfs:isDefinedBy>
        <rdfs:label>Frame Rate</rdfs:label>
    </owl:DatatypeProperty>
    


    <!-- http://dendro.fe.up.pt/ontology/tvu#genre -->

    <owl:DatatypeProperty rdf:about="http://dendro.fe.up.pt/ontology/tvu#genre">
        <rdfs:subPropertyOf rdf:resource="http://www.w3.org/2002/07/owl#topDataProperty"/>
        <rdfs:domain rdf:resource="http://dendro.fe.up.pt/ontology/tvu#AudiovisualContent"/>
        <rdfs:range rdf:resource="http://www.w3.org/2001/XMLSchema#string"/>
        <rdfs:comment>The genre of a audiovisual content (news, documentaries...)</rdfs:comment>
        <rdfs:isDefinedBy>Programmes ontology http://www.bbc.co.uk/ontologies/po</rdfs:isDefinedBy>
        <rdfs:label>Genre</rdfs:label>
    </owl:DatatypeProperty>
    


    <!-- http://dendro.fe.up.pt/ontology/tvu#height -->

    <owl:DatatypeProperty rdf:about="http://dendro.fe.up.pt/ontology/tvu#height">
        <owl:equivalentProperty rdf:resource="http://www.ebu.ch/metadata/ontologies/ebucore/ebucore#height"/>
        <rdfs:subPropertyOf rdf:resource="http://www.w3.org/2002/07/owl#topDataProperty"/>
        <rdfs:domain rdf:resource="http://dendro.fe.up.pt/ontology/tvu#AudiovisualContent"/>
        <rdfs:range rdf:resource="http://www.w3.org/2001/XMLSchema#integer"/>
        <rdfs:comment>The height of a video frame typically expressed as a number of pixels.  </rdfs:comment>
        <rdfs:isDefinedBy>EBU Ontology (ebucore) http://lov.okfn.org/dataset/lov/vocabs/ebucore</rdfs:isDefinedBy>
        <rdfs:label>Height</rdfs:label>
    </owl:DatatypeProperty>
    


    <!-- http://dendro.fe.up.pt/ontology/tvu#homepageOffice -->

    <owl:DatatypeProperty rdf:about="http://dendro.fe.up.pt/ontology/tvu#homepageOffice">
        <owl:equivalentProperty rdf:resource="http://www.ebu.ch/metadata/ontologies/ebucore/ebucore#officeHomepage"/>
        <rdfs:subPropertyOf rdf:resource="http://www.w3.org/2002/07/owl#topDataProperty"/>
        <rdfs:domain rdf:resource="http://dendro.fe.up.pt/ontology/tvu#Person"/>
        <rdfs:domain rdf:resource="http://www.w3.org/2002/07/owl#Thing"/>
        <rdfs:range rdf:resource="http://www.w3.org/2001/XMLSchema#anyURI"/>
        <rdfs:comment>Provides an office/ professional/ company web homepage of an agent (contact/ person or organization).</rdfs:comment>
        <rdfs:isDefinedBy>EBU Ontology (ebucore) http://lov.okfn.org/dataset/lov/vocabs/ebucore</rdfs:isDefinedBy>
        <rdfs:label>Homepage Office</rdfs:label>
    </owl:DatatypeProperty>
    


    <!-- http://dendro.fe.up.pt/ontology/tvu#location -->

    <owl:DatatypeProperty rdf:about="http://dendro.fe.up.pt/ontology/tvu#location">
        <rdfs:comment>The place where audiovisual content was filmed.</rdfs:comment>
        <rdfs:isDefinedBy>Programmes ontology http://www.bbc.co.uk/ontologies/po</rdfs:isDefinedBy>
        <rdfs:label>Location</rdfs:label>
    </owl:DatatypeProperty>
    


    <!-- http://dendro.fe.up.pt/ontology/tvu#locationDescription -->

    <owl:DatatypeProperty rdf:about="http://dendro.fe.up.pt/ontology/tvu#locationDescription">
        <owl:equivalentProperty rdf:resource="http://www.ebu.ch/metadata/ontologies/ebucore/ebucore#locationDescription"/>
        <rdfs:subPropertyOf rdf:resource="http://www.w3.org/2002/07/owl#topDataProperty"/>
        <rdfs:domain rdf:resource="http://dendro.fe.up.pt/ontology/tvu#AudiovisualContent"/>
        <rdfs:range rdf:resource="http://www.w3.org/2001/XMLSchema#string"/>
        <rdfs:comment>Description about the location where audiovisual content was filmed.</rdfs:comment>
        <rdfs:isDefinedBy>EBU Ontology (ebucore) http://lov.okfn.org/dataset/lov/vocabs/ebucore</rdfs:isDefinedBy>
        <rdfs:label>Location Description</rdfs:label>
    </owl:DatatypeProperty>
    


    <!-- http://dendro.fe.up.pt/ontology/tvu#numberOfFavourites -->

    <owl:DatatypeProperty rdf:about="http://dendro.fe.up.pt/ontology/tvu#numberOfFavourites">
        <rdfs:subPropertyOf rdf:resource="http://www.w3.org/2002/07/owl#topDataProperty"/>
        <rdfs:domain rdf:resource="http://dendro.fe.up.pt/ontology/tvu#AudiovisualContent"/>
        <rdfs:range rdf:resource="http://www.w3.org/2001/XMLSchema#integer"/>
        <rdfs:comment>Information about the number of users who have marked the audiovisual content as favourite.</rdfs:comment>
        <rdfs:isDefinedBy>DBpedia ontology http://wiki.dbpedia.org/services-resources/ontology</rdfs:isDefinedBy>
        <rdfs:label>Number of Favourites</rdfs:label>
    </owl:DatatypeProperty>
    


    <!-- http://dendro.fe.up.pt/ontology/tvu#numberOfVisualizations -->

    <owl:DatatypeProperty rdf:about="http://dendro.fe.up.pt/ontology/tvu#numberOfVisualizations">
        <rdfs:subPropertyOf rdf:resource="http://www.w3.org/2002/07/owl#topDataProperty"/>
        <rdfs:domain rdf:resource="http://dendro.fe.up.pt/ontology/tvu#AudiovisualContent"/>
        <rdfs:range rdf:resource="http://www.w3.org/2001/XMLSchema#integer"/>
        <rdfs:comment>Information about the number of visualizations associated to the audiovisual content.</rdfs:comment>
        <rdfs:isDefinedBy>TVU. Vocabulary</rdfs:isDefinedBy>
        <rdfs:label>Number of Visualizations</rdfs:label>
    </owl:DatatypeProperty>
    


    <!-- http://dendro.fe.up.pt/ontology/tvu#officeMailAddress -->

    <owl:DatatypeProperty rdf:about="http://dendro.fe.up.pt/ontology/tvu#officeMailAddress">
        <rdfs:subPropertyOf rdf:resource="http://www.w3.org/2002/07/owl#topDataProperty"/>
        <rdfs:domain rdf:resource="http://dendro.fe.up.pt/ontology/tvu#Person"/>
        <rdfs:domain rdf:resource="http://www.w3.org/2002/07/owl#Thing"/>
        <rdfs:range rdf:resource="http://www.w3.org/2001/XMLSchema#string"/>
        <rdfs:comment>Provides the professional/ office address of an agent (contact/ person or organization).</rdfs:comment>
        <rdfs:isDefinedBy>EBU Ontology (ebucore) http://lov.okfn.org/dataset/lov/vocabs/ebucore</rdfs:isDefinedBy>
        <rdfs:label>Office Mail Address</rdfs:label>
    </owl:DatatypeProperty>
    


    <!-- http://dendro.fe.up.pt/ontology/tvu#playbackSpeed -->

    <owl:DatatypeProperty rdf:about="http://dendro.fe.up.pt/ontology/tvu#playbackSpeed">
        <owl:equivalentProperty rdf:resource="http://www.ebu.ch/metadata/ontologies/ebucore/ebucore#playbackSpeed"/>
        <rdfs:subPropertyOf rdf:resource="http://www.w3.org/2002/07/owl#topDataProperty"/>
        <rdfs:domain rdf:resource="http://dendro.fe.up.pt/ontology/tvu#AudiovisualContent"/>
        <rdfs:range rdf:resource="http://www.w3.org/2001/XMLSchema#integer"/>
        <rdfs:comment>Identifies the rate of units against time at which the audiovisual content should be played back for human consumption. Playback speed is typically expressed in kilobit per second.</rdfs:comment>
        <rdfs:isDefinedBy>EBU Ontology (ebucore) http://lov.okfn.org/dataset/lov/vocabs/ebucore</rdfs:isDefinedBy>
        <rdfs:label>Playback Speed</rdfs:label>
    </owl:DatatypeProperty>
    


    <!-- http://dendro.fe.up.pt/ontology/tvu#publicationDate -->

    <owl:DatatypeProperty rdf:about="http://dendro.fe.up.pt/ontology/tvu#publicationDate">
        <rdfs:subPropertyOf rdf:resource="http://www.w3.org/2002/07/owl#topDataProperty"/>
        <rdfs:domain rdf:resource="http://dendro.fe.up.pt/ontology/tvu#AudiovisualContent"/>
        <rdfs:range rdf:resource="http://www.w3.org/2001/XMLSchema#integer"/>
        <rdfs:comment>The publication date of the audiovisual content.</rdfs:comment>
        <rdfs:isDefinedBy>DBpedia Ontology http://wiki.dbpedia.org/services-resources/ontology</rdfs:isDefinedBy>
        <rdfs:label>Publication Date</rdfs:label>
    </owl:DatatypeProperty>
    


    <!-- http://dendro.fe.up.pt/ontology/tvu#quotation -->

    <owl:DatatypeProperty rdf:about="http://dendro.fe.up.pt/ontology/tvu#quotation">
        <rdfs:subPropertyOf rdf:resource="http://www.w3.org/2002/07/owl#topDataProperty"/>
        <rdfs:domain rdf:resource="http://dendro.fe.up.pt/ontology/tvu#AudiovisualContent"/>
        <rdfs:range rdf:resource="http://www.w3.org/2001/XMLSchema#string"/>
        <rdfs:comment>A phrase or comment, pronounced along the audiovisual content, accompanied by the identification of the time and the author. </rdfs:comment>
        <rdfs:isDefinedBy>DBpedia Ontology http://wiki.dbpedia.org/services-resources/ontology</rdfs:isDefinedBy>
        <rdfs:label>Quotation</rdfs:label>
    </owl:DatatypeProperty>
    


    <!-- http://dendro.fe.up.pt/ontology/tvu#relatedResources -->

    <owl:DatatypeProperty rdf:about="http://dendro.fe.up.pt/ontology/tvu#relatedResources">
        <owl:equivalentProperty rdf:resource="http://www.ebu.ch/metadata/ontologies/ebucore/ebucore#relatedLink"/>
        <rdfs:subPropertyOf rdf:resource="http://www.w3.org/2002/07/owl#topDataProperty"/>
        <rdfs:domain rdf:resource="http://dendro.fe.up.pt/ontology/tvu#AudiovisualContent"/>
        <rdfs:range rdf:resource="http://www.w3.org/2001/XMLSchema#string"/>
        <rdfs:comment>A link to a web resource containing information related to a audiovisual content.</rdfs:comment>
        <rdfs:isDefinedBy>EBU Ontology (ebucore) http://lov.okfn.org/dataset/lov/vocabs/ebucore</rdfs:isDefinedBy>
        <rdfs:label>Related Resources</rdfs:label>
    </owl:DatatypeProperty>
    


    <!-- http://dendro.fe.up.pt/ontology/tvu#sampleRate -->

    <owl:DatatypeProperty rdf:about="http://dendro.fe.up.pt/ontology/tvu#sampleRate">
        <owl:equivalentProperty rdf:resource="http://www.ebu.ch/metadata/ontologies/ebucore/ebucore#sampleRate"/>
        <rdfs:subPropertyOf rdf:resource="http://www.w3.org/2002/07/owl#topDataProperty"/>
        <rdfs:domain rdf:resource="http://dendro.fe.up.pt/ontology/tvu#AudiovisualContent"/>
        <rdfs:range rdf:resource="http://www.w3.org/2001/XMLSchema#integer"/>
        <rdfs:comment>The frequency at which audio is sampled per second. Also, called sampling rate. Sample rate is usually measured in hertz ou kilohertz.</rdfs:comment>
        <rdfs:isDefinedBy>EBU Ontology (ebucore) http://lov.okfn.org/dataset/lov/vocabs/ebucore</rdfs:isDefinedBy>
        <rdfs:label>Sample Rate</rdfs:label>
    </owl:DatatypeProperty>
    


    <!-- http://dendro.fe.up.pt/ontology/tvu#samplingFormat -->

    <owl:DatatypeProperty rdf:about="http://dendro.fe.up.pt/ontology/tvu#samplingFormat">
        <owl:equivalentProperty rdf:resource="http://www.ebu.ch/metadata/ontologies/ebucore/ebucore#scanningFormat"/>
        <rdfs:subPropertyOf rdf:resource="http://www.w3.org/2002/07/owl#topDataProperty"/>
        <rdfs:domain rdf:resource="http://dendro.fe.up.pt/ontology/tvu#AudiovisualContent"/>
        <rdfs:range rdf:resource="http://www.w3.org/2001/XMLSchema#string"/>
        <rdfs:comment>Defines the scanning format for a audiovisual content. For video, the two main values are “interlaced” or “progressive”.</rdfs:comment>
        <rdfs:isDefinedBy>EBU Ontology (ebucore) http://lov.okfn.org/dataset/lov/vocabs/ebucore</rdfs:isDefinedBy>
        <rdfs:label>Sampling Format</rdfs:label>
    </owl:DatatypeProperty>
    


    <!-- http://dendro.fe.up.pt/ontology/tvu#soundField -->

    <owl:DatatypeProperty rdf:about="http://dendro.fe.up.pt/ontology/tvu#soundField">
        <rdfs:subPropertyOf rdf:resource="http://www.w3.org/2002/07/owl#topDataProperty"/>
        <rdfs:domain rdf:resource="http://dendro.fe.up.pt/ontology/tvu#AudiovisualContent"/>
        <rdfs:range rdf:resource="http://www.w3.org/2001/XMLSchema#string"/>
        <rdfs:comment>The digital sound format used in the media resource.</rdfs:comment>
        <rdfs:isDefinedBy>VideoMD: Video Technical Metadata Extension Schema http://hopewiki.socialhistoryportal.org/index.php/Media_Specific_Standards_for_Technical_Metadata</rdfs:isDefinedBy>
        <rdfs:label>Sound Field</rdfs:label>
    </owl:DatatypeProperty>
    


    <!-- http://dendro.fe.up.pt/ontology/tvu#startDateAndTime -->

    <owl:DatatypeProperty rdf:about="http://dendro.fe.up.pt/ontology/tvu#startDateAndTime">
        <rdfs:subPropertyOf rdf:resource="http://www.w3.org/2002/07/owl#topDataProperty"/>
        <rdfs:domain rdf:resource="http://dendro.fe.up.pt/ontology/tvu#AudiovisualContent"/>
        <rdfs:range rdf:resource="http://www.w3.org/2001/XMLSchema#integer"/>
        <rdfs:comment>The start date and time of an event captured in the audiovisual contents. Indicated to use in promotional media resources.</rdfs:comment>
        <rdfs:isDefinedBy>DBpedia Ontology http://wiki.dbpedia.org/services-resources/ontology</rdfs:isDefinedBy>
        <rdfs:label>Start Date and Time</rdfs:label>
    </owl:DatatypeProperty>
    


    <!-- http://dendro.fe.up.pt/ontology/tvu#telephoneOffice -->

    <owl:DatatypeProperty rdf:about="http://dendro.fe.up.pt/ontology/tvu#telephoneOffice">
        <owl:equivalentProperty rdf:resource="http://www.ebu.ch/metadata/ontologies/ebucore/ebucore#officeTelephoneNumber"/>
        <rdfs:subPropertyOf rdf:resource="http://www.w3.org/2002/07/owl#topDataProperty"/>
        <rdfs:domain rdf:resource="http://dendro.fe.up.pt/ontology/tvu#Person"/>
        <rdfs:domain rdf:resource="http://www.w3.org/2002/07/owl#Thing"/>
        <rdfs:range rdf:resource="http://www.w3.org/2001/XMLSchema#integer"/>
        <rdfs:comment>Provides an office/ professional/ telephone number of an Agent (contact/ person or organization).</rdfs:comment>
        <rdfs:isDefinedBy>EBU Ontology (ebucore) http://lov.okfn.org/dataset/lov/vocabs/ebucore</rdfs:isDefinedBy>
        <rdfs:label>Telephone Office</rdfs:label>
    </owl:DatatypeProperty>
    


    <!-- http://dendro.fe.up.pt/ontology/tvu#typeOfUpdate -->

    <owl:DatatypeProperty rdf:about="http://dendro.fe.up.pt/ontology/tvu#typeOfUpdate">
        <rdfs:subPropertyOf rdf:resource="http://www.w3.org/2002/07/owl#topDataProperty"/>
        <rdfs:domain rdf:resource="http://dendro.fe.up.pt/ontology/tvu#AudiovisualContent"/>
        <rdfs:range rdf:resource="http://www.w3.org/2001/XMLSchema#string"/>
        <rdfs:comment>Identifies the type of update which was made to a audiovisual content.</rdfs:comment>
        <rdfs:isDefinedBy>TVU. Vocabulary</rdfs:isDefinedBy>
        <rdfs:label>Type Of Update</rdfs:label>
    </owl:DatatypeProperty>
    


    <!-- http://dendro.fe.up.pt/ontology/tvu#videoMakers -->

    <owl:DatatypeProperty rdf:about="http://dendro.fe.up.pt/ontology/tvu#videoMakers">
        <rdfs:subPropertyOf rdf:resource="http://www.w3.org/2002/07/owl#topDataProperty"/>
        <rdfs:domain rdf:resource="http://dendro.fe.up.pt/ontology/tvu#AudiovisualContent"/>
        <rdfs:range rdf:resource="http://www.w3.org/2001/XMLSchema#string"/>
        <rdfs:comment>Identifies the responsibles for performing of the audiovisual contents (filming, edition work and all audience-visible components).</rdfs:comment>
        <rdfs:isDefinedBy>TVU. Vocabulary</rdfs:isDefinedBy>
        <rdfs:label>Video Makers</rdfs:label>
    </owl:DatatypeProperty>
    


    <!-- http://dendro.fe.up.pt/ontology/tvu#width -->

    <owl:DatatypeProperty rdf:about="http://dendro.fe.up.pt/ontology/tvu#width">
        <owl:equivalentProperty rdf:resource="http://www.ebu.ch/metadata/ontologies/ebucore/ebucore#width"/>
        <rdfs:subPropertyOf rdf:resource="http://www.w3.org/2002/07/owl#topDataProperty"/>
        <rdfs:domain rdf:resource="http://dendro.fe.up.pt/ontology/tvu#AudiovisualContent"/>
        <rdfs:range rdf:resource="http://www.w3.org/2001/XMLSchema#integer"/>
        <rdfs:comment>The width of a video frame typically expressed as a number of pixels.  </rdfs:comment>
        <rdfs:isDefinedBy>EBU Ontology (ebucore) http://lov.okfn.org/dataset/lov/vocabs/ebucore</rdfs:isDefinedBy>
        <rdfs:label>Width</rdfs:label>
    </owl:DatatypeProperty>
    


    <!-- http://www.ebu.ch/metadata/ontologies/ebucore/ebucore#aspectRatio -->

    <owl:DatatypeProperty rdf:about="http://www.ebu.ch/metadata/ontologies/ebucore/ebucore#aspectRatio"/>
    


    <!-- http://www.ebu.ch/metadata/ontologies/ebucore/ebucore#codecName -->

    <owl:DatatypeProperty rdf:about="http://www.ebu.ch/metadata/ontologies/ebucore/ebucore#codecName"/>
    


    <!-- http://www.ebu.ch/metadata/ontologies/ebucore/ebucore#eventDuration -->

    <owl:DatatypeProperty rdf:about="http://www.ebu.ch/metadata/ontologies/ebucore/ebucore#eventDuration"/>
    


    <!-- http://www.ebu.ch/metadata/ontologies/ebucore/ebucore#eventEndDate -->

    <owl:DatatypeProperty rdf:about="http://www.ebu.ch/metadata/ontologies/ebucore/ebucore#eventEndDate"/>
    


    <!-- http://www.ebu.ch/metadata/ontologies/ebucore/ebucore#eventStartDate -->

    <owl:DatatypeProperty rdf:about="http://www.ebu.ch/metadata/ontologies/ebucore/ebucore#eventStartDate"/>
    


    <!-- http://www.ebu.ch/metadata/ontologies/ebucore/ebucore#fileSize -->

    <owl:DatatypeProperty rdf:about="http://www.ebu.ch/metadata/ontologies/ebucore/ebucore#fileSize"/>
    


    <!-- http://www.ebu.ch/metadata/ontologies/ebucore/ebucore#filename -->

    <owl:DatatypeProperty rdf:about="http://www.ebu.ch/metadata/ontologies/ebucore/ebucore#filename"/>
    


    <!-- http://www.ebu.ch/metadata/ontologies/ebucore/ebucore#frameRate -->

    <owl:DatatypeProperty rdf:about="http://www.ebu.ch/metadata/ontologies/ebucore/ebucore#frameRate"/>
    


    <!-- http://www.ebu.ch/metadata/ontologies/ebucore/ebucore#height -->

    <owl:DatatypeProperty rdf:about="http://www.ebu.ch/metadata/ontologies/ebucore/ebucore#height"/>
    


    <!-- http://www.ebu.ch/metadata/ontologies/ebucore/ebucore#locationDescription -->

    <owl:DatatypeProperty rdf:about="http://www.ebu.ch/metadata/ontologies/ebucore/ebucore#locationDescription"/>
    


    <!-- http://www.ebu.ch/metadata/ontologies/ebucore/ebucore#officeHomepage -->

    <owl:DatatypeProperty rdf:about="http://www.ebu.ch/metadata/ontologies/ebucore/ebucore#officeHomepage"/>
    


    <!-- http://www.ebu.ch/metadata/ontologies/ebucore/ebucore#officeTelephoneNumber -->

    <owl:DatatypeProperty rdf:about="http://www.ebu.ch/metadata/ontologies/ebucore/ebucore#officeTelephoneNumber"/>
    


    <!-- http://www.ebu.ch/metadata/ontologies/ebucore/ebucore#playbackSpeed -->

    <owl:DatatypeProperty rdf:about="http://www.ebu.ch/metadata/ontologies/ebucore/ebucore#playbackSpeed"/>
    


    <!-- http://www.ebu.ch/metadata/ontologies/ebucore/ebucore#relatedLink -->

    <owl:DatatypeProperty rdf:about="http://www.ebu.ch/metadata/ontologies/ebucore/ebucore#relatedLink"/>
    


    <!-- http://www.ebu.ch/metadata/ontologies/ebucore/ebucore#sampleRate -->

    <owl:DatatypeProperty rdf:about="http://www.ebu.ch/metadata/ontologies/ebucore/ebucore#sampleRate"/>
    


    <!-- http://www.ebu.ch/metadata/ontologies/ebucore/ebucore#scanningFormat -->

    <owl:DatatypeProperty rdf:about="http://www.ebu.ch/metadata/ontologies/ebucore/ebucore#scanningFormat"/>
    


    <!-- http://www.ebu.ch/metadata/ontologies/ebucore/ebucore#width -->

    <owl:DatatypeProperty rdf:about="http://www.ebu.ch/metadata/ontologies/ebucore/ebucore#width"/>
    


    <!-- http://www.w3.org/ns/ma-ont#averageBitRate -->

    <owl:DatatypeProperty rdf:about="http://www.w3.org/ns/ma-ont#averageBitRate"/>
    


    <!-- 
    ///////////////////////////////////////////////////////////////////////////////////////
    //
    // Classes
    //
    ///////////////////////////////////////////////////////////////////////////////////////
     -->

    


    <!-- http://dendro.fe.up.pt/ontology/tvu#Actor -->

    <owl:Class rdf:about="http://dendro.fe.up.pt/ontology/tvu#Actor">
        <rdfs:subClassOf rdf:resource="http://dendro.fe.up.pt/ontology/tvu#Person"/>
        <rdfs:comment>The person who plays the role of a character in the audiovisual content.</rdfs:comment>
    </owl:Class>
    


    <!-- http://dendro.fe.up.pt/ontology/tvu#AudiovisualContent -->

    <owl:Class rdf:about="http://dendro.fe.up.pt/ontology/tvu#AudiovisualContent">
        <rdfs:subClassOf rdf:resource="http://www.w3.org/2002/07/owl#Thing"/>
        <rdfs:comment>The audiovisual content contains in the same support moving images and sound, and requires a technological device for recording, streaming, reception and understanding.</rdfs:comment>
    </owl:Class>
    


    <!-- http://dendro.fe.up.pt/ontology/tvu#Commentator -->

    <owl:Class rdf:about="http://dendro.fe.up.pt/ontology/tvu#Commentator">
        <rdfs:subClassOf rdf:resource="http://dendro.fe.up.pt/ontology/tvu#Person"/>
        <rdfs:comment>The person who relates/comments the audiovisual contents (usually in documentaries).</rdfs:comment>
    </owl:Class>
    


    <!-- http://dendro.fe.up.pt/ontology/tvu#Contributor -->

    <owl:Class rdf:about="http://dendro.fe.up.pt/ontology/tvu#Contributor">
        <rdfs:subClassOf rdf:resource="http://dendro.fe.up.pt/ontology/tvu#Person"/>
        <rdfs:comment>The entity responsible for making contributions to the audiovisual content. Examples of a contributor include an person, an organization, or an service.</rdfs:comment>
    </owl:Class>
    


    <!-- http://dendro.fe.up.pt/ontology/tvu#Creator -->

    <owl:Class rdf:about="http://dendro.fe.up.pt/ontology/tvu#Creator">
        <rdfs:subClassOf rdf:resource="http://dendro.fe.up.pt/ontology/tvu#Person"/>
        <rdfs:comment>The entity primarily responsible for making the audiovisual content.</rdfs:comment>
    </owl:Class>
    


    <!-- http://dendro.fe.up.pt/ontology/tvu#Curator -->

    <owl:Class rdf:about="http://dendro.fe.up.pt/ontology/tvu#Curator">
        <rdfs:subClassOf rdf:resource="http://dendro.fe.up.pt/ontology/tvu#Person"/>
        <rdfs:comment>The person who is responsible for making audiovisual contents available to the public and for manage the metadata associated to the audiovisual contents.</rdfs:comment>
    </owl:Class>
    


    <!-- http://dendro.fe.up.pt/ontology/tvu#Event -->

    <owl:Class rdf:about="http://dendro.fe.up.pt/ontology/tvu#Event">
        <rdfs:subClassOf rdf:resource="http://www.w3.org/2002/07/owl#Thing"/>
        <rdfs:comment>The event which is captured in the audiovisual content.</rdfs:comment>
    </owl:Class>
    


    <!-- http://dendro.fe.up.pt/ontology/tvu#Person -->

    <owl:Class rdf:about="http://dendro.fe.up.pt/ontology/tvu#Person">
        <rdfs:subClassOf rdf:resource="http://www.w3.org/2002/07/owl#Thing"/>
        <rdfs:comment>An person who have influence in the audiovisual content. It can be an actor, an commentator, an contributor, an creator, an curator or an video producer.</rdfs:comment>
    </owl:Class>
    


    <!-- http://dendro.fe.up.pt/ontology/tvu#VideoMakers -->

    <owl:Class rdf:about="http://dendro.fe.up.pt/ontology/tvu#VideoMakers">
        <rdfs:subClassOf rdf:resource="http://dendro.fe.up.pt/ontology/tvu#Person"/>
        <rdfs:comment>Identifies the responsibles for performing of the audiovisual contents (filming, edition work and all audience-visible components).</rdfs:comment>
    </owl:Class>
</rdf:RDF>



<!-- Generated by the OWL API (version 4.2.8.20170104-2310) https://github.com/owlcs/owlapi -->

