<?xml version="1.0"?>


<!DOCTYPE rdf:RDF [
    <!ENTITY owl "http://www.w3.org/2002/07/owl#" >
    <!ENTITY xsd "http://www.w3.org/2001/XMLSchema#" >
    <!ENTITY rdfs "http://www.w3.org/2000/01/rdf-schema#" >
    <!ENTITY rdf "http://www.w3.org/1999/02/22-rdf-syntax-ns#" >
]>


<rdf:RDF xmlns="http://dendro.fe.up.pt/ontology/edu#"
     xml:base="http://dendro.fe.up.pt/ontology/edu"
     xmlns:rdfs="http://www.w3.org/2000/01/rdf-schema#"
     xmlns:owl="http://www.w3.org/2002/07/owl#"
     xmlns:xsd="http://www.w3.org/2001/XMLSchema#"
     xmlns:rdf="http://www.w3.org/1999/02/22-rdf-syntax-ns#">
    <owl:Ontology rdf:about="http://dendro.fe.up.pt/ontology/socialStudies">
        <owl:imports rdf:resource="http://dendro.fe.up.pt/ontology/research"/>
        <owl:versionIRI rdf:resource="http://dendro.fe.up.pt/ontology/socialStudies/1.0"/>
    </owl:Ontology>
    


    <!-- 
    ///////////////////////////////////////////////////////////////////////////////////////
    //
    // Data properties
    //
    ///////////////////////////////////////////////////////////////////////////////////////
     -->

    


    <!-- http://dendro.fe.up.pt/ontology/socialStudies#dataCollectionDate -->

    <owl:DatatypeProperty rdf:about="http://dendro.fe.up.pt/ontology/socialStudies#dataCollectionDate">
        <rdfs:label>Data Collection Date</rdfs:label>
        <rdfs:comment>Provides a date or range of dates for the described data collection event as well as  a cycle number when the collection is part of a series of data collection events.</rdfs:comment>
        <rdfs:isDefinedBy>DDI Data Documentation Initiative (ddi:datacollection:3_2) http://www.ddialliance.org/Specification/DDI-Lifecycle/3.2/XMLSchema/FieldLevelDocumentation/namespaces/ddi_datacollection_3_2/namespace-overview.html</rdfs:isDefinedBy>
        <rdfs:subPropertyOf rdf:resource="http://purl.org/dc/terms/date"/>
    </owl:DatatypeProperty>
    


    <!-- http://dendro.fe.up.pt/ontology/socialStudies#dataCollectionMethodology -->

    <owl:DatatypeProperty rdf:about="http://dendro.fe.up.pt/ontology/socialStudies#dataCollectionMethodology">
        <rdfs:label>Data Collection Methodology</rdfs:label>
        <rdfs:isDefinedBy>DDI Data Documentation Initative (ddi:datacollection:3_2) http://www.ddialliance.org/Specification/DDI-Lifecycle/3.2/XMLSchema/FieldLevelDocumentation/schemas/datacollection_xsd/schema-overview.html</rdfs:isDefinedBy>
        <rdfs:comment>Describes the methodology used for collecting data. Repeat this element if multiple methods, or techniques, are used.</rdfs:comment>
        <rdfs:subPropertyOf rdf:resource="http://dendro.fe.up.pt/ontology/research#method"/>
    </owl:DatatypeProperty>
    


    <!-- http://dendro.fe.up.pt/ontology/socialStudies#dataCollectionSoftware -->

    <owl:DatatypeProperty rdf:about="http://dendro.fe.up.pt/ontology/socialStudies#dataCollectionSoftware">
        <rdfs:label>Data Collection Software</rdfs:label>
        <rdfs:isDefinedBy>DDI Data Documentation Initiative (ddi:datacollection:3_2) http://www.ddialliance.org/Specification/DDI-Lifecycle/3.2/XMLSchema/FieldLevelDocumentation/schemas/datacollection_xsd/schema-overview.html</rdfs:isDefinedBy>
        <rdfs:comment>Specification of a software package used to instantiate a data collection method.</rdfs:comment>
        <rdfs:subPropertyOf rdf:resource="http://dendro.fe.up.pt/ontology/research#software"/>
    </owl:DatatypeProperty>
    


    <!-- http://dendro.fe.up.pt/ontology/socialStudies#dataSource -->

    <owl:DatatypeProperty rdf:about="http://dendro.fe.up.pt/ontology/socialStudies#dataSource">
        <rdfs:label>Data Source</rdfs:label>
        <rdfs:isDefinedBy>DDI Data Documentation Initiative (ddi:datacollection:3_2) http://www.ddialliance.org/Specification/DDI-Lifecycle/3.2/XMLSchema/FieldLevelDocumentation/schemas/datacollection_xsd/schema-overview.html</rdfs:isDefinedBy>
        <rdfs:comment>Describes a source or provenance of the data.</rdfs:comment>
    </owl:DatatypeProperty>
    


    <!-- http://dendro.fe.up.pt/ontology/socialStudies#externalAid -->

    <owl:DatatypeProperty rdf:about="http://dendro.fe.up.pt/ontology/socialStudies#externalAid">
        <rdfs:label>External Aid</rdfs:label>
        <rdfs:isDefinedBy>DDI Data Documentation Initiative (ddi:datacollection:3_2)
http://www.ddialliance.org/Specification/DDI-Lifecycle/3.2/XMLSchema/FieldLevelDocumentation/schemas/datacollection_xsd/schema-overview.html</rdfs:isDefinedBy>
        <rdfs:comment>A pointer to an external aid presented by the instrument such as a text card, image, audio, or audiovisual aid. Typically a URN. Use type attribute to describe the type of external aid provided. Example of terms to use would include: imageOnly audioOnly audioVisual multiMedia.</rdfs:comment>
        <rdfs:subPropertyOf rdf:resource="&owl;topDataProperty"/>
    </owl:DatatypeProperty>
    


    <!-- http://dendro.fe.up.pt/ontology/socialStudies#kindOfData -->

    <owl:DatatypeProperty rdf:about="http://dendro.fe.up.pt/ontology/socialStudies#kindOfData">
        <rdfs:label>Kind Of Data</rdfs:label>
        <rdfs:comment>Briefly describes the kind of data documented in the logical product(s) of a group unit. Examples include survey data, census/enumeration data, administrative data, measurement data, assessment data, demographic data, voting data, etc. Admissible values are &quot;Qualitative&quot; | &quot;Quantitative&quot; | &quot;Mixed&quot;</rdfs:comment>
        <rdfs:isDefinedBy>DDI Data documentation initiative (ddi:reusable:3_2) http://www.ddialliance.org/Specification/DDI-Lifecycle/3.2/XMLSchema/FieldLevelDocumentation/</rdfs:isDefinedBy>
        <rdfs:range rdf:resource="&xsd;string"/>
    </owl:DatatypeProperty>
    


    <!-- http://dendro.fe.up.pt/ontology/socialStudies#methodology -->

    <owl:DatatypeProperty rdf:about="http://dendro.fe.up.pt/ontology/socialStudies#methodology">
        <rdfs:label>Methodology</rdfs:label>
        <rdfs:comment>Metadata regarding the methodologies used concerning data collection, determining the timing and repetition patterns for data collection, and sampling procedures.</rdfs:comment>
        <rdfs:isDefinedBy>DDI Data Documentation Initiative (ddi:datacollection:3_2)
http://www.ddialliance.org/Specification/DDI-Lifecycle/3.2/XMLSchema/FieldLevelDocumentation/schemas/datacollection_xsd/schema-overview.html</rdfs:isDefinedBy>
        <rdfs:subPropertyOf rdf:resource="http://dendro.fe.up.pt/ontology/research#method"/>
    </owl:DatatypeProperty>
    


    <!-- http://dendro.fe.up.pt/ontology/socialStudies#sampleSize -->

    <owl:DatatypeProperty rdf:about="http://dendro.fe.up.pt/ontology/socialStudies#sampleSize">
        <rdfs:label>Sample Size</rdfs:label>
        <rdfs:comment>The size of the sample from whom data was requested.</rdfs:comment>
        <rdfs:isDefinedBy>Data Documentation Initiative (ddi:datacollection:3_2)
http://www.ddialliance.org/Specification/DDI-Lifecycle/3.2/XMLSchema/FieldLevelDocumentation/namespaces/ddi_datacollection_3_2/namespace-overview.html</rdfs:isDefinedBy>
        <rdfs:subPropertyOf rdf:resource="http://dendro.fe.up.pt/ontology/research#measurement"/>
        <rdfs:range rdf:resource="&xsd;integer"/>
    </owl:DatatypeProperty>
    


    <!-- http://dendro.fe.up.pt/ontology/socialStudies#samplingProcedure -->

    <owl:DatatypeProperty rdf:about="http://dendro.fe.up.pt/ontology/socialStudies#samplingProcedure">
        <rdfs:label>Sampling Procedure</rdfs:label>
        <rdfs:isDefinedBy>DDI Data Documentation Initiative (ddi:datacollection:3_2) http://www.ddialliance.org/Specification/DDI-Lifecycle/3.2/XMLSchema/FieldLevelDocumentation/</rdfs:isDefinedBy>
        <rdfs:comment>Describes the type of sample, sample design and provides details on drawing the sample. May be repeated to provide descriptions of individual facets of a single sample design or when multiple sampling methods are used. When multiple descriptions are used, the use of a controlled vocabulary to identify the parts and relationships is strongly recommended.</rdfs:comment>
        <rdfs:subPropertyOf rdf:resource="http://dendro.fe.up.pt/ontology/research#method"/>
    </owl:DatatypeProperty>
    


    <!-- http://dendro.fe.up.pt/ontology/socialStudies#universe -->

    <owl:DatatypeProperty rdf:about="http://dendro.fe.up.pt/ontology/socialStudies#universe">
        <rdfs:label>Universe</rdfs:label>
        <rdfs:isDefinedBy>DDI Data documentation initiative (ddi:reusable:3_2)
http://www.ddialliance.org/Specification/DDI-Lifecycle/3.2/XMLSchema/FieldLevelDocumentation/namespaces/ddi_conceptualcomponent_3_2/namespace-overview.html</rdfs:isDefinedBy>
        <rdfs:comment>Describes a universe which may also be known as a population.</rdfs:comment>
    </owl:DatatypeProperty>
    


    <!-- http://purl.org/dc/terms/date -->

    <owl:DatatypeProperty rdf:about="http://purl.org/dc/terms/date"/>
    


    <!-- 
    ///////////////////////////////////////////////////////////////////////////////////////
    //
    // Classes
    //
    ///////////////////////////////////////////////////////////////////////////////////////
     -->

    


    <!-- http://dendro.fe.up.pt/ontology/socialStudies#BehaviouralStudy -->

    <owl:Class rdf:about="http://dendro.fe.up.pt/ontology/socialStudies#BehaviouralStudy">
        <rdfs:subClassOf rdf:resource="http://dendro.fe.up.pt/ontology/research#ResearchAsset"/>
    </owl:Class>
</rdf:RDF>



<!-- Generated by the OWL API (version 3.4.2) http://owlapi.sourceforge.net -->

