@prefix owl: <http://www.w3.org/2002/07/owl#> .
@prefix rdfs: <http://www.w3.org/2000/01/rdf-schema#> .
@prefix dc11: <http://purl.org/dc/elements/1.1/> .
@prefix dc: <http://purl.org/dc/terms/> .
@prefix ns0: <http://www.bbc.co.uk/ontologies/provenance/> .
@prefix xsd: <http://www.w3.org/2001/XMLSchema#> .
@prefix ns1: <http://www.w3.org/2003/06/sw-vocab-status/ns#> .
@prefix foaf: <http://xmlns.com/foaf/0.1/> .
@prefix geo: <http://www.w3.org/2003/01/geo/wgs84_pos#> .

<http://purl.org/ontology/po/>
  a <http://www.bbc.co.uk/ontologies/provenance/Ontology>, owl:Ontology ;
  rdfs:comment """
		A vocabulary for programme data.
		It defines concepts such as brands, series, episodes, broadcasts, etc.
	""" ;
  rdfs:isDefinedBy <http://purl.org/ontology/po/> ;
  rdfs:label "Programmes ontology" ;
  dc11:contributor <http://metade.org/foaf.rdf#me>, <http://www.aelius.com/njh#me>, <http://smethur.st/#me> ;
  dc11:creator <http://moustaki.org/foaf.rdf#moustaki> ;
  dc11:date "2009/02/20 16:00:00" ;
  dc:license <http://creativecommons.org/licenses/by/4.0#id> ;
  ns0:canonicalLocation "https://repo.dev.bbc.co.uk/services/linked-data/ontologies/domain/programmes"^^xsd:string ;
  ns0:changeReason "Adding contributor"@en-gb ;
  ns0:public true ;
  ns0:slug "po"^^xsd:string ;
  ns0:version "1.1"^^xsd:string ;
  owl:imports <http://purl.org/NET/c4dm/event.owl>, <http://purl.org/NET/c4dm/timeline.owl>, dc11:, dc:, <http://www.bbc.co.uk/ontologies/provenance> ;
  owl:priorVersion <http://purl.org/ontology/po/1.0> ;
  owl:versionIRI <http://purl.org/ontology/po/1.1> ;
  owl:versionInfo "1.1"^^xsd:string .

<http://purl.org/ontology/po/AudioDescribedVersion>
  a owl:Class ;
  rdfs:comment """
		A version holding an audio description.
	""" ;
  rdfs:isDefinedBy <http://purl.org/ontology/po/> ;
  rdfs:label "AudioDescribedVersion" ;
  rdfs:subClassOf <http://purl.org/ontology/po/Version> ;
  ns1:term_status "testing" .

<http://purl.org/ontology/po/Brand>
  a owl:Class ;
  rdfs:comment """
		A brand, e.g. `Top Gear'
	""" ;
  rdfs:isDefinedBy <http://purl.org/ontology/po/> ;
  rdfs:label "Brand" ;
  rdfs:subClassOf <http://purl.org/ontology/po/Programme> ;
  owl:disjointWith <http://purl.org/ontology/po/Clip>, <http://purl.org/ontology/po/Episode>, <http://purl.org/ontology/po/Series> ;
  ns1:term_status "stable" .

<http://purl.org/ontology/po/Broadcast>
  a owl:Class ;
  rdfs:comment """
		A broadcast event.
		Subsumes the event concept defined in
		the Event ontology.
		A broadcast is associated with a service, and with a
		particular version of an episode.
	""" ;
  rdfs:isDefinedBy <http://purl.org/ontology/po/> ;
  rdfs:label "Broadcast" ;
  rdfs:subClassOf <http://purl.org/NET/c4dm/event.owl#Event> ;
  ns1:term_status "stable" .

<http://purl.org/ontology/po/Broadcaster>
  a owl:Class ;
  rdfs:comment """
		An organization responsible of some broadcasting services.
        It can hold a set of services and outlets.
	""" ;
  rdfs:isDefinedBy <http://purl.org/ontology/po/> ;
  rdfs:label "Broadcaster" ;
  rdfs:subClassOf foaf:Organization ;
  ns1:term_status "stable" .

<http://purl.org/ontology/po/Category>
  a owl:Class ;
  rdfs:comment """
        A category provides a way of classifying a set of programmes. Such classifications
        can be performed according to multiple dimensions and taxonomies, e.g. genre, format, places, people, subjects...
    """ ;
  rdfs:isDefinedBy <http://purl.org/ontology/po/> ;
  rdfs:label "Category" ;
  ns1:term_status "testing" .

<http://purl.org/ontology/po/Channel>
  a owl:Class ;
  rdfs:comment """
        A physical channel on which a broadcast occurs.
        A single outlet or service can be associated with multiple channels.
        For example, Radio 4 LW broadcasts on Analogue Long Wave and on Digital
        Satellite.
    """ ;
  rdfs:isDefinedBy <http://purl.org/ontology/po/> ;
  rdfs:label "Channel" ;
  ns1:term_status "testing" .

<http://purl.org/ontology/po/Clip>
  a owl:Class ;
  rdfs:comment """
        A particular clip, e.g. `Clip of Top Gear, first series'
    """ ;
  rdfs:isDefinedBy <http://purl.org/ontology/po/> ;
  rdfs:label "Clip" ;
  rdfs:subClassOf <http://purl.org/ontology/po/Programme>, <http://purl.org/ontology/po/ProgrammeItem> ;
  owl:disjointWith <http://purl.org/ontology/po/Brand>, <http://purl.org/ontology/po/Series> ;
  ns1:term_status "testing" .

<http://purl.org/ontology/po/DAB>
  a owl:Class ;
  rdfs:comment """
		Digital Audio Broadcasting
	""" ;
  rdfs:isDefinedBy <http://purl.org/ontology/po/> ;
  rdfs:label "DAB" ;
  rdfs:subClassOf <http://purl.org/ontology/po/Channel> ;
  ns1:term_status "testing" .

<http://purl.org/ontology/po/DVB>
  a owl:Class ;
  rdfs:comment """
		Digital Video Broadcasting
	""" ;
  rdfs:isDefinedBy <http://purl.org/ontology/po/> ;
  rdfs:label "DVB" ;
  rdfs:subClassOf <http://purl.org/ontology/po/Channel> ;
  ns1:term_status "testing" .

<http://purl.org/ontology/po/Episode>
  a owl:Class ;
  rdfs:comment """
		A particular episode, e.g. `Top Gear, first episode of the first series' or the film 'A Walk in the Sun' (http://www.bbc.co.uk/programmes/b00gfzdt)
	""" ;
  rdfs:isDefinedBy <http://purl.org/ontology/po/> ;
  rdfs:label "Episode" ;
  rdfs:subClassOf <http://purl.org/ontology/po/Programme>, <http://purl.org/ontology/po/ProgrammeItem> ;
  owl:disjointWith <http://purl.org/ontology/po/Brand>, <http://purl.org/ontology/po/Series> ;
  ns1:term_status "stable" .

<http://purl.org/ontology/po/FM>
  a owl:Class ;
  rdfs:comment """
		The FM broadcast band
	""" ;
  rdfs:isDefinedBy <http://purl.org/ontology/po/> ;
  rdfs:label "FM" ;
  rdfs:subClassOf <http://purl.org/ontology/po/Channel> ;
  ns1:term_status "testing" .

<http://purl.org/ontology/po/FirstBroadcast>
  a owl:Class ;
  rdfs:comment """
		Specifies a broadcast as being the
		first one of a particular version.
	 """ ;
  rdfs:isDefinedBy <http://purl.org/ontology/po/> ;
  rdfs:label "FirstBroadcast" ;
  rdfs:subClassOf <http://purl.org/ontology/po/Broadcast> ;
  owl:disjointWith <http://purl.org/ontology/po/RepeatBroadcast> ;
  ns1:term_status "testing" .

<http://purl.org/ontology/po/Format>
  a owl:Class ;
  rdfs:comment """
        Anchor point for format taxonomies, similar to po:Genre for genre taxonomies.
        Instances of this concept include documentaries, talk shows, animation, etc.
    """ ;
  rdfs:isDefinedBy <http://purl.org/ontology/po/> ;
  rdfs:label "Format" ;
  rdfs:subClassOf <http://purl.org/ontology/po/Category> ;
  ns1:term_status "testing" .

<http://purl.org/ontology/po/Genre>
  a owl:Class ;
  rdfs:comment """
        An anchor point for a programmes' genre taxonomy, e.g. 'Drama'/'Biographical'.
	""" ;
  rdfs:isDefinedBy <http://purl.org/ontology/po/> ;
  rdfs:label "Genre" ;
  rdfs:subClassOf <http://purl.org/ontology/po/Category> ;
  ns1:term_status "testing" .

<http://purl.org/ontology/po/IPStream>
  a owl:Class ;
  rdfs:comment """
		IP stream
	""" ;
  rdfs:isDefinedBy <http://purl.org/ontology/po/> ;
  rdfs:label "IP stream" ;
  rdfs:subClassOf <http://purl.org/ontology/po/Channel> ;
  ns1:term_status "testing" .

<http://purl.org/ontology/po/LW>
  a owl:Class ;
  rdfs:comment """
		The AM broadcast band
	""" ;
  rdfs:isDefinedBy <http://purl.org/ontology/po/> ;
  rdfs:label "AM" ;
  rdfs:subClassOf <http://purl.org/ontology/po/Channel> ;
  ns1:term_status "testing" .

<http://purl.org/ontology/po/LocalRadio>
  a owl:Class ;
  rdfs:comment """
		Radio services aiming at a local coverage.
	""" ;
  rdfs:isDefinedBy <http://purl.org/ontology/po/> ;
  rdfs:label "LocalRadio" ;
  rdfs:subClassOf <http://purl.org/ontology/po/Radio> ;
  owl:disjointWith <http://purl.org/ontology/po/NationalRadio>, <http://purl.org/ontology/po/RegionalRadio> ;
  ns1:term_status "testing" .

<http://purl.org/ontology/po/MusicSegment>
  a owl:Class ;
  rdfs:comment """
		Classification of an episode version's region corresponding to a musical track being played.
	""" ;
  rdfs:label "MusicSegment" ;
  rdfs:subClassOf <http://purl.org/ontology/po/Segment> ;
  ns1:term_status "testing" .

<http://purl.org/ontology/po/NationalRadio>
  a owl:Class ;
  rdfs:comment """
		Radio services aiming at a national coverage.
	""" ;
  rdfs:isDefinedBy <http://purl.org/ontology/po/> ;
  rdfs:label "NationalRadio"^^xsd:string ;
  rdfs:subClassOf <http://purl.org/ontology/po/Radio> ;
  ns1:term_status "testing" .

<http://purl.org/ontology/po/OriginalVersion>
  a owl:Class ;
  rdfs:comment """
		An `original' version, the legacy version of
		a particular episode.
	""" ;
  rdfs:isDefinedBy <http://purl.org/ontology/po/> ;
  rdfs:label "OriginalVersion"^^xsd:string ;
  rdfs:subClassOf <http://purl.org/ontology/po/Version> ;
  owl:disjointWith <http://purl.org/ontology/po/ShortenedVersion> ;
  ns1:term_status "testing" .

<http://purl.org/ontology/po/Outlet>
  a owl:Class ;
  rdfs:comment """
        Outlet of a particular service, e.g. Radio 4 LW and FM for Radio 4.
        Outlets are services which do not have variations.
        The criterion for an outlet is its timeline.
        For example, Radio 4 LW broadcasts on Analogue Long Wave, but also on Digital Satellite.
        It corresponds to just one outlet, as they are simulcasts.
        The two physical channels for broadcasts correspond to po:Channel.
    """ ;
  rdfs:isDefinedBy <http://purl.org/ontology/po/> ;
  rdfs:label "Outlet"^^xsd:string ;
  rdfs:subClassOf <http://purl.org/ontology/po/Service> ;
  ns1:term_status "testing" .

<http://purl.org/ontology/po/Person>
  a owl:Class ;
  rdfs:comment "A person" ;
  rdfs:isDefinedBy <http://purl.org/ontology/po/> ;
  rdfs:label "Person"^^xsd:string ;
  rdfs:subClassOf <http://purl.org/ontology/po/Category> ;
  owl:equivalentClass foaf:Person ;
  ns1:term_status "testing" .

<http://purl.org/ontology/po/Place>
  a owl:Class ;
  rdfs:comment "A physical place" ;
  rdfs:isDefinedBy <http://purl.org/ontology/po/> ;
  rdfs:label "Place"^^xsd:string ;
  rdfs:subClassOf <http://purl.org/ontology/po/Category> ;
  owl:equivalentClass geo:Feature ;
  ns1:term_status "testing" .

<http://purl.org/ontology/po/Programme>
  a owl:Class ;
  rdfs:comment """
		A programme, can either be a brand, a series or an episode
	""" ;
  rdfs:isDefinedBy <http://purl.org/ontology/po/> ;
  rdfs:label "Programme"^^xsd:string ;
  ns1:term_status "stable" .

<http://purl.org/ontology/po/ProgrammeItem>
  a owl:Class ;
  rdfs:comment """
        A programme that can have versions, and as such can be broadcast or made available on-demand, e.g. a clip or an episode.
    """ ;
  rdfs:isDefinedBy <http://purl.org/ontology/po/> ;
  rdfs:label "ProgrammeItem"^^xsd:string ;
  rdfs:subClassOf <http://purl.org/ontology/po/Programme> ;
  owl:disjointWith <http://purl.org/ontology/po/Brand>, <http://purl.org/ontology/po/Series> ;
  ns1:term_status "testing" .

<http://purl.org/ontology/po/Radio>
  a owl:Class ;
  rdfs:comment """
		Services that use a radio medium.
	""" ;
  rdfs:isDefinedBy <http://purl.org/ontology/po/> ;
  rdfs:label "Radio"^^xsd:string ;
  rdfs:subClassOf <http://purl.org/ontology/po/Service> ;
  owl:disjointWith <http://purl.org/ontology/po/TV>, <http://purl.org/ontology/po/Web> ;
  ns1:term_status "testing" .

<http://purl.org/ontology/po/RegionalRadio>
  a owl:Class ;
  rdfs:comment """
		Radio services aiming at a regional coverage.
	""" ;
  rdfs:isDefinedBy <http://purl.org/ontology/po/> ;
  rdfs:label "RegionalRadio"^^xsd:string ;
  rdfs:subClassOf <http://purl.org/ontology/po/Radio> ;
  owl:disjointWith <http://purl.org/ontology/po/NationalRadio> ;
  ns1:term_status "testing" .

<http://purl.org/ontology/po/RepeatBroadcast>
  a owl:Class ;
  rdfs:comment """
		Specifies a broadcast as being a
		repeat.
	""" ;
  rdfs:isDefinedBy <http://purl.org/ontology/po/> ;
  rdfs:label "Repeat"^^xsd:string ;
  rdfs:subClassOf <http://purl.org/ontology/po/Broadcast> ;
  owl:disjointWith <http://purl.org/ontology/po/FirstBroadcast> ;
  ns1:term_status "testing" .

<http://purl.org/ontology/po/Season>
  a owl:Class ;
  rdfs:comment """
		A season is a group of broadcasts.
	""" ;
  rdfs:isDefinedBy <http://purl.org/ontology/po/> ;
  rdfs:label "Season"^^xsd:string ;
  ns1:term_status "testing" .

<http://purl.org/ontology/po/Segment>
  a owl:Class ;
  rdfs:comment """
		Classification of an episode version's region, e.g. 'this track was played at that time'.
	""" ;
  rdfs:isDefinedBy <http://purl.org/ontology/po/> ;
  rdfs:label "Segment"^^xsd:string ;
  rdfs:subClassOf <http://purl.org/NET/c4dm/event.owl#Event> ;
  ns1:term_status "testing" .

<http://purl.org/ontology/po/Series>
  a owl:Class ;
  rdfs:comment """
		A series, e.g. `Top Gear, first season'
	""" ;
  rdfs:isDefinedBy <http://purl.org/ontology/po/> ;
  rdfs:label "Series"^^xsd:string ;
  rdfs:subClassOf <http://purl.org/ontology/po/Programme> ;
  ns1:term_status "stable" .

<http://purl.org/ontology/po/Service>
  a owl:Class ;
  rdfs:comment """
        A broadcasting service.
		Instances of this concept include BBC Radio Wales, BBC Radio 4, BBC News, etc.
        A service is a collection of outlets which contain common material, but with some variations, e.g. by
        region.
        Hence, a service may have multiple outlets (po:Outlet), e.g. BBC Radio 4 has BBC Radio 4 LW and BBC Radio 4 FM.
        A hierarchy of services types is defined within this ontology, e.g. radio and TV.
        A service that is a master brand only (a service that only commissions programmes, e.g. BBC Switch) should
        be an instance of the top-level po:Service.
	""" ;
  rdfs:isDefinedBy <http://purl.org/ontology/po/> ;
  rdfs:label "Service"^^xsd:string ;
  ns1:term_status "stable" .

<http://purl.org/ontology/po/ShortenedVersion>
  a owl:Class ;
  rdfs:comment """
		A shortened version.
	""" ;
  rdfs:isDefinedBy <http://purl.org/ontology/po/> ;
  rdfs:label "ShortenedVersion"^^xsd:string ;
  rdfs:subClassOf <http://purl.org/ontology/po/Version> ;
  owl:disjointWith <http://purl.org/ontology/po/OriginalVersion> ;
  ns1:term_status "testing" .

<http://purl.org/ontology/po/SignedVersion>
  a owl:Class ;
  rdfs:comment """
		A version holding sign language.
	""" ;
  rdfs:isDefinedBy <http://purl.org/ontology/po/> ;
  rdfs:label "SignLanguage"^^xsd:string ;
  rdfs:subClassOf <http://purl.org/ontology/po/Version> ;
  ns1:term_status "testing" .

<http://purl.org/ontology/po/SpeechSegment>
  a owl:Class ;
  rdfs:comment """
        Classification of an episode version's region holding speech content.
    """ ;
  rdfs:subClassOf <http://purl.org/ontology/po/Segment> ;
  ns1:term_status "testing" .

<http://purl.org/ontology/po/Subject>
  a owl:Class ;
  rdfs:comment """
        Anchor point for subject taxonomies.
    """ ;
  rdfs:isDefinedBy <http://purl.org/ontology/po/> ;
  rdfs:label "Subject"^^xsd:string ;
  rdfs:subClassOf <http://purl.org/ontology/po/Category> ;
  ns1:term_status "testing" .

<http://purl.org/ontology/po/Subtitle>
  a owl:Class ;
  rdfs:comment """
        Classification of an episode version's region corresponding to a subtitle being shown.
    """ ;
  rdfs:isDefinedBy <http://purl.org/ontology/po/> ;
  rdfs:label "Subtitle"^^xsd:string ;
  rdfs:subClassOf <http://purl.org/NET/c4dm/event.owl#Event> ;
  ns1:term_status "testing" .

<http://purl.org/ontology/po/TV>
  a owl:Class ;
  rdfs:comment """
		Services that use a television medium.
	""" ;
  rdfs:isDefinedBy <http://purl.org/ontology/po/> ;
  rdfs:label "TV"^^xsd:string ;
  rdfs:subClassOf <http://purl.org/ontology/po/Service> ;
  owl:disjointWith <http://purl.org/ontology/po/Web> ;
  ns1:term_status "testing" .

<http://purl.org/ontology/po/Version>
  a owl:Class ;
  rdfs:comment """
		A particular version of an episode.
		Such versions include shortened ones, audio described ones
		or ones that holds sign language.
		The version is associated to a timeline.
	""" ;
  rdfs:isDefinedBy <http://purl.org/ontology/po/> ;
  rdfs:label "Version"^^xsd:string ;
  ns1:term_status "stable" .

<http://purl.org/ontology/po/Web>
  a owl:Class ;
  rdfs:comment """
		Services that use a Web medium.
	""" ;
  rdfs:isDefinedBy <http://purl.org/ontology/po/> ;
  rdfs:label "Web"^^xsd:string ;
  rdfs:subClassOf <http://purl.org/ontology/po/Service> ;
  ns1:term_status "testing" .

<http://purl.org/ontology/po/actor>
  a owl:ObjectProperty ;
  rdfs:comment "Relates a programmes to one of its actors - a person who plays the role of a character" ;
  rdfs:domain <http://purl.org/ontology/po/Programme> ;
  rdfs:isDefinedBy <http://purl.org/ontology/po/> ;
  rdfs:label "actor" ;
  rdfs:range foaf:Agent ;
  rdfs:subPropertyOf <http://purl.org/ontology/po/credit> ;
  ns1:term_status "testing" .

<http://purl.org/ontology/po/anchor>
  a owl:ObjectProperty ;
  rdfs:comment "A television reporter who coordinates a programme" ;
  rdfs:domain <http://purl.org/ontology/po/Programme> ;
  rdfs:isDefinedBy <http://purl.org/ontology/po/> ;
  rdfs:label "anchor" ;
  rdfs:range foaf:Agent ;
  rdfs:subPropertyOf <http://purl.org/ontology/po/credit> ;
  ns1:term_status "testing" .

<http://purl.org/ontology/po/aspect_ratio>
  a owl:DatatypeProperty ;
  rdfs:comment """
		The aspect ration of a particular version.
	""" ;
  rdfs:domain <http://purl.org/ontology/po/Version> ;
  rdfs:isDefinedBy <http://purl.org/ontology/po/> ;
  rdfs:label "aspect ratio" ;
  rdfs:range xsd:string ;
  ns1:term_status "testing" .

<http://purl.org/ontology/po/author>
  a owl:ObjectProperty ;
  rdfs:comment "Relates a programme to its author - the person who created the content" ;
  rdfs:domain <http://purl.org/ontology/po/Programme> ;
  rdfs:isDefinedBy <http://purl.org/ontology/po/> ;
  rdfs:label "author" ;
  rdfs:range foaf:Agent ;
  rdfs:subPropertyOf <http://purl.org/ontology/po/credit> ;
  ns1:term_status "testing" .

<http://purl.org/ontology/po/broadcast_of>
  a owl:ObjectProperty ;
  rdfs:comment """
		Relates a particular broadcast to the version being broadcasted.
		Sub-property of the event:factor one.
	""" ;
  rdfs:domain <http://purl.org/ontology/po/Broadcast> ;
  rdfs:isDefinedBy <http://purl.org/ontology/po/> ;
  rdfs:label "broadcast of" ;
  rdfs:range <http://purl.org/ontology/po/Version> ;
  rdfs:subPropertyOf <http://purl.org/NET/c4dm/event.owl#factor> ;
  ns1:term_status "testing" .

<http://purl.org/ontology/po/broadcast_on>
  a owl:ObjectProperty ;
  rdfs:comment """
		Relates a particular broadcast to the service or outlet on which it was.
		Sub-property of the event:factor one.
	""" ;
  rdfs:domain <http://purl.org/ontology/po/Broadcast> ;
  rdfs:isDefinedBy <http://purl.org/ontology/po/> ;
  rdfs:label "broadcast on" ;
  rdfs:range <http://purl.org/ontology/po/Service> ;
  rdfs:subPropertyOf <http://purl.org/NET/c4dm/event.owl#factor> ;
  owl:equivalentProperty <http://purl.org/ontology/po/broadcasted_on> ;
  ns1:term_status "testing" .

<http://purl.org/ontology/po/broadcasted_on>
  a owl:ObjectProperty ;
  rdfs:comment "Deprecated property, left here for historical reasons" .

<http://purl.org/ontology/po/broadcaster>
  a owl:ObjectProperty ;
  rdfs:comment """
		Associates a service to a broadcaster
	""" ;
  rdfs:domain <http://purl.org/ontology/po/Service> ;
  rdfs:isDefinedBy <http://purl.org/ontology/po/> ;
  rdfs:label "broadcaster" ;
  rdfs:range <http://purl.org/ontology/po/Broadcaster> ;
  ns1:term_status "testing" .

<http://purl.org/ontology/po/category>
  a owl:ObjectProperty ;
  rdfs:comment """
        Relates a programme to a particular category, e.g. genre, format, place...
    """ ;
  rdfs:domain <http://purl.org/ontology/po/Programme> ;
  rdfs:isDefinedBy <http://purl.org/ontology/po/> ;
  rdfs:label "category" ;
  rdfs:range <http://purl.org/ontology/po/Genre> ;
  ns1:term_status "testing" .

<http://purl.org/ontology/po/channel>
  a owl:ObjectProperty ;
  rdfs:comment """
        Associates a service to a channel, e.g. Radio 4 LW to Radio 4 LW on Analogue Long Wave.
    """ ;
  rdfs:domain <http://purl.org/ontology/po/Service> ;
  rdfs:isDefinedBy <http://purl.org/ontology/po/> ;
  rdfs:label "channel" ;
  rdfs:range <http://purl.org/ontology/po/Channel> ;
  ns1:term_status "testing" .

<http://purl.org/ontology/po/clip>
  a owl:ObjectProperty ;
  rdfs:comment """
        Associates a brand, a series or an episode to a clip.
    """ ;
  rdfs:isDefinedBy <http://purl.org/ontology/po/> ;
  rdfs:label "clip" ;
  rdfs:range <http://purl.org/ontology/po/Clip> ;
  rdfs:subPropertyOf dc:hasPart ;
  ns1:term_status "testing" .

<http://purl.org/ontology/po/commentator>
  a owl:ObjectProperty ;
  rdfs:comment "Relates a programme to one of its commentators" ;
  rdfs:domain <http://purl.org/ontology/po/Programme> ;
  rdfs:isDefinedBy <http://purl.org/ontology/po/> ;
  rdfs:label "commentator" ;
  rdfs:range foaf:Agent ;
  rdfs:subPropertyOf <http://purl.org/ontology/po/credit> ;
  ns1:term_status "testing" .

<http://purl.org/ontology/po/credit>
  a owl:ObjectProperty ;
  rdfs:comment "Relates a programmes to a person who is credited in it" ;
  rdfs:domain <http://purl.org/ontology/po/Programme> ;
  rdfs:isDefinedBy <http://purl.org/ontology/po/> ;
  rdfs:label "credit" ;
  rdfs:range foaf:Agent ;
  rdfs:subPropertyOf dc11:contributor ;
  ns1:term_status "testing" .

<http://purl.org/ontology/po/director>
  a owl:ObjectProperty ;
  rdfs:comment "Relates a programme to its supervisor. Generally refers to the person responsible for all audience-visible components of a program, film, or show, whereas the producer is responsible for the financial and other behind-the-scenes aspects. A director's duties might also include casting, script editing, shot selection, shot composition, and editing" ;
  rdfs:domain <http://purl.org/ontology/po/Programme> ;
  rdfs:isDefinedBy <http://purl.org/ontology/po/> ;
  rdfs:label "director" ;
  rdfs:range foaf:Agent ;
  rdfs:subPropertyOf <http://purl.org/ontology/po/credit> ;
  ns1:term_status "testing" .

<http://purl.org/ontology/po/duration>
  a owl:DatatypeProperty ;
  rdfs:comment "The duration of a version, in seconds." ;
  rdfs:isDefinedBy <http://purl.org/ontology/po/> ;
  rdfs:label "duration" ;
  rdfs:range xsd:int ;
  ns1:term_status "testing" .

<http://purl.org/ontology/po/episode>
  a owl:ObjectProperty ;
  rdfs:comment """
		Associates a brand or a series to an episode constituting it.
	""" ;
  rdfs:isDefinedBy <http://purl.org/ontology/po/> ;
  rdfs:label "episode" ;
  rdfs:range <http://purl.org/ontology/po/Episode> ;
  rdfs:subPropertyOf dc:hasPart ;
  ns1:term_status "testing" .

<http://purl.org/ontology/po/executive_producer>
  a owl:ObjectProperty ;
  rdfs:comment "Relates a programme to its executive producer - a producer who is not involved in any technical aspects of the making process, but who is still responsible for the overall production. Typically an executive producer handles business and legal issues" ;
  rdfs:domain <http://purl.org/ontology/po/Programme> ;
  rdfs:isDefinedBy <http://purl.org/ontology/po/> ;
  rdfs:label "executive producer" ;
  rdfs:range foaf:Agent ;
  rdfs:subPropertyOf <http://purl.org/ontology/po/credit> ;
  ns1:term_status "testing" .

<http://purl.org/ontology/po/format>
  a owl:ObjectProperty ;
  rdfs:comment """
		Relates a programme to a particular format (eg. `Animation', `Documentary', etc.).
	""" ;
  rdfs:domain <http://purl.org/ontology/po/Programme> ;
  rdfs:isDefinedBy <http://purl.org/ontology/po/> ;
  rdfs:label "format" ;
  rdfs:range <http://purl.org/ontology/po/Format> ;
  rdfs:subPropertyOf <http://purl.org/ontology/po/category> ;
  ns1:term_status "testing" .

<http://purl.org/ontology/po/frequency>
  a owl:DatatypeProperty ;
  rdfs:comment "Associates a channel to its frequency" ;
  rdfs:domain <http://purl.org/ontology/po/Channel> ;
  rdfs:isDefinedBy <http://purl.org/ontology/po/> ;
  rdfs:label "frequency" ;
  rdfs:range xsd:float ;
  ns1:term_status "testing" .

<http://purl.org/ontology/po/genre>
  a owl:ObjectProperty ;
  rdfs:comment """
		Relates a programme to a particular genre.
	""" ;
  rdfs:domain <http://purl.org/ontology/po/Programme> ;
  rdfs:isDefinedBy <http://purl.org/ontology/po/> ;
  rdfs:label "genre" ;
  rdfs:range <http://purl.org/ontology/po/Genre> ;
  rdfs:subPropertyOf <http://purl.org/ontology/po/category> ;
  ns1:term_status "testing" .

<http://purl.org/ontology/po/location>
  a owl:ObjectProperty ;
  rdfs:comment """
		Associates a service to a geographic location,
		aiming at capturing what this service aims at covering.
	""" ;
  rdfs:domain <http://purl.org/ontology/po/Service> ;
  rdfs:isDefinedBy <http://purl.org/ontology/po/> ;
  rdfs:label "location" ;
  rdfs:range geo:SpatialThing ;
  rdfs:subPropertyOf foaf:based_near ;
  ns1:term_status "testing" .

<http://purl.org/ontology/po/long_synopsis>
  a owl:DatatypeProperty ;
  rdfs:comment """
		A long synopsis of a series, brand or episode.
		Sub-property of po:synopsis.
	""" ;
  rdfs:isDefinedBy <http://purl.org/ontology/po/> ;
  rdfs:label "long synopsis" ;
  rdfs:subPropertyOf <http://purl.org/ontology/po/synopsis> ;
  ns1:term_status "testing" .

<http://purl.org/ontology/po/masterbrand>
  a owl:ObjectProperty ;
  rdfs:comment "Associates a programme with its masterbrand (its commissioner)" ;
  rdfs:domain <http://purl.org/ontology/po/Programme> ;
  rdfs:isDefinedBy <http://purl.org/ontology/po/> ;
  rdfs:label "masterbrand" ;
  rdfs:range <http://purl.org/ontology/po/Service> ;
  ns1:term_status "stable" .

<http://purl.org/ontology/po/medium_synopsis>
  a owl:DatatypeProperty ;
  rdfs:comment """
		A medium synopsis of a series, brand or episode.
		Sub-property of po:synopsis.
	""" ;
  rdfs:isDefinedBy <http://purl.org/ontology/po/> ;
  rdfs:label "medium synopsis" ;
  rdfs:subPropertyOf <http://purl.org/ontology/po/synopsis> ;
  ns1:term_status "testing" .

<http://purl.org/ontology/po/microsite>
  a owl:ObjectProperty ;
  rdfs:comment "Associates a programme to its microsite. For example http://www.bbc.co.uk/programmes/b00fm04s and http://www.bbc.co.uk/eastenders/" ;
  rdfs:domain <http://purl.org/ontology/po/Programme> ;
  rdfs:isDefinedBy <http://purl.org/ontology/po/> ;
  rdfs:label "microsite" ;
  rdfs:range foaf:Document ;
  rdfs:subPropertyOf foaf:page ;
  ns1:term_status "testing" .

<http://purl.org/ontology/po/news_reader>
  a owl:ObjectProperty ;
  rdfs:comment "Relates a programme to its news reader" ;
  rdfs:domain <http://purl.org/ontology/po/Programme> ;
  rdfs:isDefinedBy <http://purl.org/ontology/po/> ;
  rdfs:label "news reader" ;
  rdfs:range foaf:Agent ;
  rdfs:subPropertyOf <http://purl.org/ontology/po/credit> ;
  ns1:term_status "testing" .

<http://purl.org/ontology/po/outlet>
  a owl:ObjectProperty ;
  rdfs:comment """
		Associates a service to an outlet, e.g. Radio 4 to Radio 4 LW.
	""" ;
  rdfs:domain <http://purl.org/ontology/po/Service> ;
  rdfs:isDefinedBy <http://purl.org/ontology/po/> ;
  rdfs:label "outlet" ;
  rdfs:range <http://purl.org/ontology/po/Outlet> ;
  ns1:term_status "testing" .

<http://purl.org/ontology/po/parent_series>
  a owl:ObjectProperty, owl:TransitiveProperty ;
  rdfs:comment """
		Relates a series to a series constituting it (eg. `Waking the dead').
	""" ;
  rdfs:domain <http://purl.org/ontology/po/Series> ;
  rdfs:isDefinedBy <http://purl.org/ontology/po/> ;
  rdfs:label "parent series" ;
  rdfs:range <http://purl.org/ontology/po/Series> ;
  rdfs:subPropertyOf dc:isPartOf ;
  ns1:term_status "testing" .

<http://purl.org/ontology/po/parent_service>
  a owl:ObjectProperty, owl:TransitiveProperty ;
  rdfs:comment """
		Relates a service to another service encapsulating it (eg. `BBC One' and `BBC One South')
	""" ;
  rdfs:domain <http://purl.org/ontology/po/Service> ;
  rdfs:isDefinedBy <http://purl.org/ontology/po/> ;
  rdfs:label "parent service" ;
  rdfs:range <http://purl.org/ontology/po/Service> ;
  rdfs:subPropertyOf dc:isPartOf ;
  ns1:term_status "testing" .

<http://purl.org/ontology/po/participant>
  a owl:ObjectProperty ;
  rdfs:comment "Relates a programme to one of its participants" ;
  rdfs:domain <http://purl.org/ontology/po/Programme> ;
  rdfs:isDefinedBy <http://purl.org/ontology/po/> ;
  rdfs:label "participant" ;
  rdfs:range foaf:Agent ;
  rdfs:subPropertyOf <http://purl.org/ontology/po/credit> ;
  ns1:term_status "testing" .

<http://purl.org/ontology/po/performer>
  a owl:ObjectProperty ;
  rdfs:comment "Relates a programme to an entertainer who performs a dramatic or musical work for audience" ;
  rdfs:domain <http://purl.org/ontology/po/Programme> ;
  rdfs:isDefinedBy <http://purl.org/ontology/po/> ;
  rdfs:label "performer" ;
  rdfs:range foaf:Agent ;
  rdfs:subPropertyOf <http://purl.org/ontology/po/credit> ;
  ns1:term_status "testing" .

<http://purl.org/ontology/po/person>
  a owl:ObjectProperty ;
  rdfs:comment """
        Relates a programme to a person
    """ ;
  rdfs:domain <http://purl.org/ontology/po/Programme> ;
  rdfs:isDefinedBy <http://purl.org/ontology/po/> ;
  rdfs:label "person" ;
  rdfs:range <http://purl.org/ontology/po/Person> ;
  rdfs:subPropertyOf <http://purl.org/ontology/po/category> ;
  ns1:term_status "testing" .

<http://purl.org/ontology/po/place>
  a owl:ObjectProperty ;
  rdfs:comment """
        Relates a programme to a place (e.g. `London')
    """ ;
  rdfs:domain <http://purl.org/ontology/po/Programme> ;
  rdfs:isDefinedBy <http://purl.org/ontology/po/> ;
  rdfs:label "place" ;
  rdfs:range <http://purl.org/ontology/po/Place> ;
  rdfs:subPropertyOf <http://purl.org/ontology/po/category> ;
  ns1:term_status "testing" .

<http://purl.org/ontology/po/position>
  a owl:DatatypeProperty ;
  rdfs:comment "The position of a particular series or episode within its containing programme. This property can also be used to give the position of an interval within the containing timeline." ;
  rdfs:isDefinedBy <http://purl.org/ontology/po/> ;
  rdfs:label "position" ;
  rdfs:range xsd:int ;
  ns1:term_status "testing" .

<http://purl.org/ontology/po/producer>
  a owl:ObjectProperty ;
  rdfs:comment "Relates a programme to its producer - the manager of an event, show, or other work, usually the individual in charge of finance, personnel, and other non-artistic aspects in the development of commercials, plays, movies, and other works" ;
  rdfs:domain <http://purl.org/ontology/po/Programme> ;
  rdfs:isDefinedBy <http://purl.org/ontology/po/> ;
  rdfs:label "producer" ;
  rdfs:range foaf:Agent ;
  rdfs:subPropertyOf <http://purl.org/ontology/po/credit> ;
  ns1:term_status "testing" .

<http://purl.org/ontology/po/schedule_date>
  a owl:DatatypeProperty ;
  rdfs:comment """
		The schedule date of a broadcast event.
	""" ;
  rdfs:domain <http://purl.org/ontology/po/Broadcast> ;
  rdfs:isDefinedBy <http://purl.org/ontology/po/> ;
  rdfs:label "schedule date" ;
  rdfs:range xsd:date ;
  ns1:term_status "testing" .

<http://purl.org/ontology/po/season_broadcast>
  a owl:ObjectProperty ;
  rdfs:comment "Associates a season to its constituent broadcasts" ;
  rdfs:domain <http://purl.org/ontology/po/Season> ;
  rdfs:isDefinedBy <http://purl.org/ontology/po/> ;
  rdfs:label "broadcast" ;
  rdfs:range <http://purl.org/ontology/po/Broadcast> ;
  ns1:term_status "testing" .

<http://purl.org/ontology/po/series>
  a owl:ObjectProperty, owl:TransitiveProperty ;
  rdfs:comment """
		Associates a brand or a series to a series constituting it.
	""" ;
  rdfs:isDefinedBy <http://purl.org/ontology/po/> ;
  rdfs:label "series" ;
  rdfs:range <http://purl.org/ontology/po/Series> ;
  rdfs:subPropertyOf dc:hasPart ;
  ns1:term_status "testing" .

<http://purl.org/ontology/po/service>
  a owl:FunctionalProperty, owl:ObjectProperty ;
  rdfs:comment """
		Associate a brand, series or episode to the master brand service.
	""" ;
  rdfs:domain <http://purl.org/ontology/po/Programme> ;
  rdfs:isDefinedBy <http://purl.org/ontology/po/> ;
  rdfs:label "service" ;
  rdfs:range <http://purl.org/ontology/po/Service> ;
  ns1:term_status "testing" .

<http://purl.org/ontology/po/short_synopsis>
  a owl:DatatypeProperty ;
  rdfs:comment """
		A short synopsis of a series, brand or episode.
		Sub-property of po:synopsis.
	""" ;
  rdfs:isDefinedBy <http://purl.org/ontology/po/> ;
  rdfs:label "short synopsis" ;
  rdfs:subPropertyOf <http://purl.org/ontology/po/synopsis> ;
  ns1:term_status "testing" .

<http://purl.org/ontology/po/sound_format>
  a owl:DatatypeProperty ;
  rdfs:comment """
		The sound format of a particular version.
	""" ;
  rdfs:domain <http://purl.org/ontology/po/Version> ;
  rdfs:isDefinedBy <http://purl.org/ontology/po/> ;
  rdfs:label "sound format" ;
  rdfs:range xsd:string ;
  ns1:term_status "testing" .

<http://purl.org/ontology/po/subject>
  a owl:ObjectProperty ;
  rdfs:comment """
        Relates a programme to a subject (e.g. `Easter')
    """ ;
  rdfs:domain <http://purl.org/ontology/po/Programme> ;
  rdfs:isDefinedBy <http://purl.org/ontology/po/> ;
  rdfs:label "subject" ;
  rdfs:range <http://purl.org/ontology/po/Subject> ;
  rdfs:subPropertyOf <http://purl.org/ontology/po/category> ;
  ns1:term_status "testing" .

<http://purl.org/ontology/po/subtitle_language>
  a owl:DatatypeProperty ;
  rdfs:comment "Language of the subtitles embedded in a particular version" ;
  rdfs:domain <http://purl.org/ontology/po/Version> ;
  rdfs:isDefinedBy <http://purl.org/ontology/po/> ;
  rdfs:label "subtitle language" ;
  rdfs:range xsd:string ;
  ns1:term_status "testing" .

<http://purl.org/ontology/po/synopsis>
  a owl:DatatypeProperty ;
  rdfs:comment """
		The synopsis of a series, brand or episode.
	""" ;
  rdfs:domain <http://purl.org/ontology/po/Programme> ;
  rdfs:isDefinedBy <http://purl.org/ontology/po/> ;
  rdfs:label "synopsis" ;
  rdfs:range xsd:string ;
  ns1:term_status "testing" .

<http://purl.org/ontology/po/text>
  a owl:DatatypeProperty ;
  rdfs:comment "Associates a subtitle event to the corresponding text" ;
  rdfs:domain <http://purl.org/ontology/po/Subtitle> ;
  rdfs:isDefinedBy <http://purl.org/ontology/po/> ;
  rdfs:label "text" ;
  rdfs:range xsd:string ;
  ns1:term_status "testing" .

<http://purl.org/ontology/po/time>
  a owl:ObjectProperty ;
  rdfs:comment "Associates an episode's version or a version's segment with a temporal interval. This interval can be associated with a timeline, serving as an anchor for further temporal annotations, e.g. subtitles or played track" ;
  rdfs:isDefinedBy <http://purl.org/ontology/po/> ;
  rdfs:label "time" ;
  rdfs:range <http://purl.org/NET/c4dm/timeline.owl#Interval> ;
  ns1:term_status "stable" .

<http://purl.org/ontology/po/track>
  a owl:ObjectProperty ;
  rdfs:comment "Associates a music segment with a track, as defined in MO" ;
  rdfs:domain <http://purl.org/ontology/po/MusicSegment> ;
  rdfs:isDefinedBy <http://purl.org/ontology/po/> ;
  rdfs:label "track" ;
  rdfs:range <http://purl.org/ontology/mo/Track> ;
  rdfs:subPropertyOf <http://purl.org/NET/c4dm/event.owl#factor> ;
  ns1:term_status "testing" .

<http://purl.org/ontology/po/version>
  a owl:InverseFunctionalProperty, owl:ObjectProperty ;
  rdfs:comment """
		Associate an episode to a version of it.
		Different versions of a same episode can exist (shortened version, version
		designed for the hearing impaired, etc.).
	""" ;
  rdfs:domain <http://purl.org/ontology/po/ProgrammeItem> ;
  rdfs:isDefinedBy <http://purl.org/ontology/po/> ;
  rdfs:label "version" ;
  rdfs:range <http://purl.org/ontology/po/Version> ;
  ns1:term_status "testing" .
